Seperate signatures in SHA3.Vec modules

code/sha3/Hacl.Impl.SHA3.Vec.fst
@@ -1,41 +1,17 @@
 module Hacl.Impl.SHA3.Vec
 
-open Hacl.Spec.SHA3.Vec.Common
-
-open FStar.HyperStack.All
-open FStar.HyperStack
-open FStar.HyperStack.ST
-open FStar.Mul
-open Lib.IntTypes
-open Lib.NTuple
-open Lib.Sequence
 open Lib.IntVector
-open Lib.MultiBuffer
-open Lib.LoopCombinators
 open Lib.IntVector.Transpose
-
-open LowStar.Buffer
-open LowStar.BufferOps
-
-open Lib.IntTypes
 open Lib.Buffer
-open Lib.ByteBuffer
 
-open Spec.Hash.Definitions
 open Spec.SHA3.Constants
 
-open Hacl.Spec.SHA3.Vec
-
 module ST = FStar.HyperStack.ST
-module B = LowStar.Buffer
 module LSeq = Lib.Sequence
-module LB = Lib.ByteSequence
 module Loop = Lib.LoopCombinators
-module S = Spec.SHA3
-module Equiv = Spec.SHA3.Equivalence
 module V = Hacl.Spec.SHA3.Vec
-module HD = Hacl.Hash.Definitions
 
+inline_for_extraction noextract
 let disjoint4_4 #len1 #len2 #a (b0 b1 b2 b3: lbuffer a len1) (b4 b5 b6 b7: lbuffer a len2) =
   disjoint b0 b4 /\ disjoint b0 b5 /\ disjoint b0 b6 /\ disjoint b0 b7 /\
   disjoint b1 b4 /\ disjoint b1 b5 /\ disjoint b1 b6 /\ disjoint b1 b7 /\
@@ -51,54 +27,12 @@ private let keccak_piln :x:glbuffer piln_t 24ul{witnessed x keccak_piln /\ recal
 private let keccak_rndc :x:glbuffer pub_uint64 24ul{witnessed x keccak_rndc /\ recallable x}
   = createL_global rndc_list
 
-#set-options "--z3rlimit 50 --fuel 0 --ifuel 0"
+#set-options "--z3rlimit 80 --fuel 0 --ifuel 0"
 
-inline_for_extraction noextract
-let state_t (m:m_spec) = lbuffer (element_t m) 25ul
-
-inline_for_extraction noextract
-let ws_t (m:m_spec) = lbuffer (element_t m) 32ul
-
-inline_for_extraction noextract
-let index = n:size_t{v n < 5}
-
-inline_for_extraction noextract
-val get:
-    m:m_spec
-  -> s:state_t m
-  -> x:index
-  -> y:index
-  -> Stack (element_t m)
-    (requires fun h -> live h s)
-    (ensures  fun h0 r h1 ->
-      modifies loc_none h0 h1 /\
-      r == V.get m (as_seq h0 s) (v x) (v y))
 let get _ s x y = s.(x +! 5ul *! y)
 
-inline_for_extraction noextract
-val set:
-    m:m_spec
-  -> s:state_t m
-  -> x:index
-  -> y:index
-  -> v:element_t m
-  -> Stack unit
-    (requires fun h -> live h s)
-    (ensures  fun h0 _ h1 ->
-      modifies (loc s) h0 h1 /\
-      as_seq h1 s == V.set m (as_seq h0 s) (size_v x) (size_v y) v)
 let set _ s x y v = s.(x +! 5ul *! y) <- v
 
-inline_for_extraction noextract
-val state_theta0:
-    m:m_spec
-  -> s:state_t m
-  -> _C:lbuffer (element_t m) 5ul
-  -> Stack unit
-    (requires fun h -> live h s /\ live h _C /\ disjoint _C s)
-    (ensures  fun h0 _ h1 ->
-      modifies (loc _C) h0 h1 /\
-      as_seq h1 _C == V.state_theta0 m (as_seq h0 s) (as_seq h0 _C))
 let state_theta0 m s _C =
   [@ inline_let]
   let spec h0 = V.state_theta_inner_C m (as_seq h0 s) in
@@ -114,17 +48,6 @@ let state_theta0 m s _C =
       get m s x 4ul
   )
 
-inline_for_extraction noextract
-val state_theta_inner_s:
-    m:m_spec
-  -> _C:lbuffer (element_t m) 5ul
-  -> x:index
-  -> s:state_t m
-  -> Stack unit
-    (requires fun h0 -> live h0 s /\ live h0 _C /\ disjoint _C s)
-    (ensures  fun h0 _ h1 ->
-      modifies (loc s) h0 h1 /\
-      as_seq h1 s == V.state_theta_inner_s m (as_seq h0 _C) (v x) (as_seq h0 s))
 let state_theta_inner_s m _C x s =
   let _D = _C.((x +. 4ul) %. 5ul) ^| (_C.((x +. 1ul) %. 5ul) <<<| 1ul) in
   [@ inline_let]
@@ -136,16 +59,6 @@ let state_theta_inner_s m _C x s =
     set m s x y (get m s x y ^| _D)
   )
 
-inline_for_extraction noextract
-val state_theta1:
-    m:m_spec
-  -> s:state_t m
-  -> _C:lbuffer (element_t m) 5ul
-  -> Stack unit
-    (requires fun h0 -> live h0 s /\ live h0 _C /\ disjoint _C s)
-    (ensures  fun h0 _ h1 ->
-      modifies (loc s) h0 h1 /\
-      as_seq h1 s == V.state_theta1 m (as_seq h0 _C) (as_seq h0 s))
 let state_theta1 m s _C =
   [@ inline_let]
   let spec h0 = V.state_theta_inner_s m (as_seq h0 _C) in
@@ -156,22 +69,12 @@ let state_theta1 m s _C =
     state_theta_inner_s m _C x s
   )
 
-inline_for_extraction noextract
-val state_theta:
-    m:m_spec
-  -> s:state_t m
-  -> Stack unit
-    (requires fun h -> live h s)
-    (ensures  fun h0 _ h1 ->
-      modifies (loc s) h0 h1 /\
-      as_seq h1 s == V.state_theta m (as_seq h0 s))
 let state_theta m s =
   push_frame ();
   let h0 = ST.get() in
   let _C = create 5ul (zero_element m) in 
   state_theta0 m s _C; state_theta1 m s _C;
   pop_frame()
-
 
 #reset-options "--max_fuel 1 --max_ifuel 1 --z3rlimit 50"
 
@@ -187,19 +90,6 @@ let rec index_map #a #b f l i =
 
 #reset-options "--max_fuel 0 --max_ifuel 0 --z3rlimit 100"
 
-inline_for_extraction noextract
-val state_pi_rho_inner:
-    m:m_spec
-  -> i:size_t{v i < 24}
-  -> current:lbuffer (element_t m) 1ul
-  -> s:state_t m
-  -> Stack unit
-    (requires fun h -> live h s /\ live h current /\ disjoint current s)
-    (ensures  fun h0 _ h1 ->
-      modifies (loc_union (loc s) (loc current)) h0 h1 /\
-      (let c', s' = V.state_pi_rho_inner m (v i) (bget h0 current 0, as_seq h0 s) in
-      bget h1 current 0 == c' /\
-      as_seq h1 s == s'))
 let state_pi_rho_inner _ i current s =
   assert_norm (List.Tot.length piln_list == 24);
   let h0 = ST.get () in
@@ -212,15 +102,6 @@ let state_pi_rho_inner _ i current s =
   s.(_Y) <- current.(0ul) <<<| r;
   current.(0ul) <- temp
 
-inline_for_extraction noextract
-val state_pi_rho:
-    m:m_spec
-  -> s:state_t m
-  -> Stack unit
-    (requires fun h -> live h s)
-    (ensures  fun h0 _ h1 ->
-      modifies (loc s) h0 h1 /\
-      as_seq h1 s == V.state_pi_rho m (as_seq h0 s))
 let state_pi_rho m s =
   push_frame();
   let x = get m s 1ul 0ul in
@@ -242,16 +123,6 @@ let state_pi_rho m s =
   );
   pop_frame()
 
-inline_for_extraction noextract
-val state_chi_inner:
-    m:m_spec
-  -> st:state_t m
-  -> y:index
-  -> Stack unit
-    (requires fun h0 -> live h0 st)
-    (ensures  fun h0 _ h1 ->
-      modifies (loc st) h0 h1 /\
-      as_seq h1 st == V.state_chi_inner m (v y) (as_seq h0 st))
 let state_chi_inner m st y =
   let h0 = ST.get() in
   let v0  = get m st 0ul y ^| ((~| (get m st 1ul y)) &| get m st 2ul y) in
@@ -268,15 +139,6 @@ let state_chi_inner m st y =
   assert (modifies (loc st) h0 h1);
   assert (as_seq h1 st == V.state_chi_inner m (v y) (as_seq h0 st))
 
-inline_for_extraction noextract
-val state_chi:
-    m:m_spec
-  -> s:state_t m
-  -> Stack unit
-    (requires fun h -> live h s)
-    (ensures  fun h0 _ h1 ->
-      modifies (loc s) h0 h1 /\
-      as_seq h1 s == V.state_chi m (as_seq h0 s))
 let state_chi m st =
   let h0 = ST.get() in
   [@ inline_let]
@@ -291,30 +153,11 @@ let state_chi m st =
   assert(as_seq h1 st == V.state_chi_equiv m (as_seq h0 st));
   V.state_chi_equivalence m (as_seq h0 st)
 
-inline_for_extraction noextract
-val state_iota:
-    m:m_spec
-  -> s:state_t m
-  -> round:size_t{v round < 24}
-  -> Stack unit
-    (requires fun h -> live h s)
-    (ensures  fun h0 _ h1 ->
-      modifies (loc s) h0 h1 /\
-      as_seq h1 s == V.state_iota m (as_seq h0 s) (v round))
 let state_iota m s round =
   recall_contents keccak_rndc Spec.SHA3.Constants.keccak_rndc;
   let c = keccak_rndc.(round) in
   set m s 0ul 0ul (get m s 0ul 0ul ^| (load_element m (secret c)))
 
-inline_for_extraction noextract
-val state_permute:
-    m:m_spec
-  -> s:state_t m
-  -> Stack unit
-    (requires fun h -> live h s)
-    (ensures  fun h0 _ h1 ->
-      modifies (loc s) h0 h1 /\
-      as_seq h1 s == V.state_permute m (as_seq h0 s))
 let state_permute m s =
   [@ inline_let]
   let spec h0 = V.state_permute1 m in
@@ -327,24 +170,13 @@ let state_permute m s =
     state_chi m s;
     state_iota m s round)
 
-inline_for_extraction noextract
-val set_wsi: #a:keccak_alg -> #m:m_spec
-  -> ws:ws_t m
-  -> i:size_t{v i < 32}
-  -> b:lbuffer uint8 256ul
-  -> bi:size_t{v bi < 32 / (lanes m)} ->
-  Stack unit
-  (requires fun h -> live h b /\ live h ws /\ disjoint b ws)
-  (ensures  fun h0 _ h1 -> modifies (loc ws) h0 h1 /\
-    as_seq h1 ws == LSeq.upd (as_seq h0 ws) (v i) (V.load_elementi #a #m (as_seq h0 b) (v bi)))
-
 let set_wsi #a #m ws i b bi =
   [@inline_let]
   let l = lanes m in
   ws.(i) <- vec_load_le (word_t a) l (sub b (bi *! size l *! 8ul) (size l *! 8ul))
 
 noextract
-let load_blocks_spec1 (#a:keccak_alg) (#m:m_spec{lanes m == 1}) (b:multiblock_spec a m) : ws_spec m =
+let load_blocks_spec1 (#a:keccak_alg) (#m:m_spec{lanes m == 1}) (b:V.multiblock_spec a m) : V.ws_spec m =
   let b = b.(|0|) in
   let ws0 = V.load_elementi #a #m b 0 in
   let ws1 = V.load_elementi #a #m b 1 in
@@ -384,28 +216,10 @@ let load_blocks_spec1 (#a:keccak_alg) (#m:m_spec{lanes m == 1}) (b:multiblock_sp
            ws24 ws25 ws26 ws27 ws28 ws29 ws30 ws31
 
 noextract
-let load_blocks_spec1_lemma (#a:keccak_alg) (#m:m_spec{lanes m == 1}) (b:multiblock_spec a m) :
+let load_blocks_spec1_lemma (#a:keccak_alg) (#m:m_spec{lanes m == 1}) (b:V.multiblock_spec a m) :
   Lemma (V.load_blocks b == load_blocks_spec1 b)
  =
   LSeq.eq_intro (V.load_blocks b) (load_blocks_spec1 b)
-
-inline_for_extraction noextract
-val set_wsi_1_4: #a:keccak_alg -> #m:m_spec{lanes m == 1}
-  -> ws:ws_t m
-  -> i:size_t{v i < 32 /\ v (i +! 3ul) < 32}
-  -> b:lbuffer uint8 256ul
-  -> bi:size_t{v bi < 32 / (lanes m) /\ v (bi +! 3ul) < 32 / (lanes m)} ->
-  Stack unit
-  (requires fun h -> live h b /\ live h ws /\ disjoint b ws)
-  (ensures  fun h0 _ h1 -> modifies (loc ws) h0 h1 /\
-    (let ws1 = as_seq h1 ws in
-     let ws0 = as_seq h0 ws in
-     ws1.[v i + 0] == V.load_elementi #a #m (as_seq h0 b) (v bi + 0) /\
-     ws1.[v i + 1] == V.load_elementi #a #m (as_seq h0 b) (v bi + 1) /\
-     ws1.[v i + 2] == V.load_elementi #a #m (as_seq h0 b) (v bi + 2) /\
-     ws1.[v i + 3] == V.load_elementi #a #m (as_seq h0 b) (v bi + 3) /\
-     (forall (j: nat). j < v i ==> ws1.[j] == ws0.[j]) /\
-     (forall (j: nat). j >= v i + 4 /\ j < 32 ==> ws1.[j] == ws0.[j])))
 
 let set_wsi_1_4 #a #m ws i b bi =
   set_wsi #a #m ws i b bi;
@@ -413,19 +227,18 @@ let set_wsi_1_4 #a #m ws i b bi =
   set_wsi #a #m ws (i+!2ul) b (bi+!2ul);
   set_wsi #a #m ws (i+!3ul) b (bi+!3ul)
 
-inline_for_extraction noextract
-val load_blocks1: #a:keccak_alg -> #m:m_spec{lanes m == 1}
-  -> b:multibuf (lanes m) 256ul
-  -> ws:ws_t m ->
-  Stack unit
-  (requires fun h -> live_multi h b /\ live h ws /\ disjoint_multi b ws)
-  (ensures  fun h0 _ h1 -> modifies (loc ws) h0 h1 /\
-    as_seq h1 ws == V.load_blocks #a #m (as_seq_multi h0 b))
-
-#push-options "--z3rlimit 200"
+#push-options "--max_fuel 1 --z3rlimit 200"
 let load_blocks1 #a #m ib ws =
   let h0 = ST.get() in
-  let b = ib.(|0|) in
+  assert (v (0ul +! 3ul) == 3);
+  assert (v (4ul +! 3ul) == 7);
+  assert (v (8ul +! 3ul) == 11);
+  assert (v (12ul +! 3ul) == 15);
+  assert (v (16ul +! 3ul) == 19);
+  assert (v (20ul +! 3ul) == 23);
+  assert (v (24ul +! 3ul) == 27);
+  assert (v (28ul +! 3ul) == 31);
+  let b = tup1 ib in
   set_wsi_1_4 #a #m ws 0ul b 0ul;
   set_wsi_1_4 #a #m ws 4ul b 4ul;
   set_wsi_1_4 #a #m ws 8ul b 8ul;
@@ -443,7 +256,7 @@ let load_blocks1 #a #m ib ws =
 #pop-options
 
 noextract
-let load_blocks_spec4 (#a:keccak_alg) (#m:m_spec{lanes m == 4}) (b:multiblock_spec a m) : ws_spec m =
+let load_blocks_spec4 (#a:keccak_alg) (#m:m_spec{lanes m == 4}) (b:V.multiblock_spec a m) : V.ws_spec m =
   let b0 = b.(|0|) in
   let b1 = b.(|1|) in
   let b2 = b.(|2|) in
@@ -486,32 +299,10 @@ let load_blocks_spec4 (#a:keccak_alg) (#m:m_spec{lanes m == 4}) (b:multiblock_sp
            ws24 ws25 ws26 ws27 ws28 ws29 ws30 ws31
 
 noextract
-let load_blocks_spec4_lemma (#a:keccak_alg) (#m:m_spec{lanes m == 4}) (b:multiblock_spec a m) :
+let load_blocks_spec4_lemma (#a:keccak_alg) (#m:m_spec{lanes m == 4}) (b:V.multiblock_spec a m) :
   Lemma (V.load_blocks b == load_blocks_spec4 b)
  =
   LSeq.eq_intro (V.load_blocks b) (load_blocks_spec4 b)
-
-inline_for_extraction noextract
-val set_wsi_4_4: #a:keccak_alg -> #m:m_spec{lanes m == 4}
-  -> ws:ws_t m
-  -> i:size_t{v i < 32 /\ v (i +! 3ul) < 32}
-  -> b0:lbuffer uint8 256ul
-  -> b1:lbuffer uint8 256ul
-  -> b2:lbuffer uint8 256ul
-  -> b3:lbuffer uint8 256ul
-  -> bi:size_t{v bi < 32 / (lanes m)} ->
-  Stack unit
-  (requires fun h -> live h b0 /\ live h b1 /\ live h b2 /\ live h b3 /\
-    live h ws /\ disjoint b0 ws /\ disjoint b1 ws /\ disjoint b2 ws /\ disjoint b3 ws)
-  (ensures  fun h0 _ h1 -> modifies (loc ws) h0 h1 /\
-    (let ws1 = as_seq h1 ws in
-     let ws0 = as_seq h0 ws in
-     ws1.[v i + 0] == V.load_elementi #a #m (as_seq h0 b0) (v bi) /\
-     ws1.[v i + 1] == V.load_elementi #a #m (as_seq h0 b1) (v bi) /\
-     ws1.[v i + 2] == V.load_elementi #a #m (as_seq h0 b2) (v bi) /\
-     ws1.[v i + 3] == V.load_elementi #a #m (as_seq h0 b3) (v bi) /\
-     (forall (j: nat). j < v i ==> ws1.[j] == ws0.[j]) /\
-     (forall (j: nat). j >= v i + 4 /\ j < 32 ==> ws1.[j] == ws0.[j])))
 
 let set_wsi_4_4 #a #m ws i b0 b1 b2 b3 bi =
   set_wsi #a #m ws i b0 bi;
@@ -519,18 +310,17 @@ let set_wsi_4_4 #a #m ws i b0 b1 b2 b3 bi =
   set_wsi #a #m ws (i+!2ul) b2 bi;
   set_wsi #a #m ws (i+!3ul) b3 bi
 
-inline_for_extraction noextract
-val load_blocks4: #a:keccak_alg -> #m:m_spec{lanes m == 4}
-  -> b:multibuf (lanes m) 256ul
-  -> ws:ws_t m ->
-  Stack unit
-  (requires fun h -> live_multi h b /\ live h ws /\ disjoint_multi b ws)
-  (ensures  fun h0 _ h1 -> modifies (loc ws) h0 h1 /\
-    as_seq h1 ws == V.load_blocks #a #m (as_seq_multi h0 b))
-
-#push-options "--z3rlimit 200"
+#push-options "--max_fuel 1 --z3rlimit 200"
 let load_blocks4 #a #m ib ws =
   let h0 = ST.get() in
+  assert (v (0ul +! 3ul) == 3);
+  assert (v (4ul +! 3ul) == 7);
+  assert (v (8ul +! 3ul) == 11);
+  assert (v (12ul +! 3ul) == 15);
+  assert (v (16ul +! 3ul) == 19);
+  assert (v (20ul +! 3ul) == 23);
+  assert (v (24ul +! 3ul) == 27);
+  assert (v (28ul +! 3ul) == 31);
   let (b0,(b1,(b2,b3))) = tup4 ib in
   set_wsi_4_4 #a #m ws 0ul b0 b1 b2 b3 0ul;
   set_wsi_4_4 #a #m ws 4ul b0 b1 b2 b3 1ul;
@@ -549,28 +339,10 @@ let load_blocks4 #a #m ib ws =
   ()
 #pop-options
 
-inline_for_extraction noextract
-val load_blocks: #a:keccak_alg -> #m:m_spec{is_supported m}
-  -> b:multibuf (lanes m) 256ul
-  -> ws:ws_t m ->
-  Stack unit
-  (requires fun h -> live_multi h b /\ live h ws /\ disjoint_multi b ws)
-  (ensures  fun h0 _ h1 -> modifies (loc ws) h0 h1 /\
-    as_seq h1 ws == V.load_blocks #a #m (as_seq_multi h0 b))
-
 let load_blocks #a #m b ws =
   match lanes m with
   | 1 -> load_blocks1 #a #m b ws
   | 4 -> load_blocks4 #a #m b ws
-
-inline_for_extraction noextract
-val transpose_ws4:
-    #m:m_spec{lanes m == 4}
-  -> ws:ws_t m
-  -> Stack unit
-    (requires fun h -> live h ws)
-    (ensures  fun h0 _ h1 -> modifies (loc ws) h0 h1 /\
-      as_seq h1 ws == V.transpose_ws (as_seq h0 ws))
 
 let transpose_ws4 #m ws =
   let (ws0,ws1,ws2,ws3) =
@@ -592,46 +364,19 @@ let transpose_ws4 #m ws =
   create32 ws ws0 ws1 ws2 ws3 ws4 ws5 ws6 ws7 ws8 ws9 ws10 ws11 ws12 ws13 ws14 ws15
     ws16 ws17 ws18 ws19 ws20 ws21 ws22 ws23 ws24 ws25 ws26 ws27 ws28 ws29 ws30 ws31
 
-inline_for_extraction noextract
-val transpose_ws: #m:m_spec{is_supported m} -> ws:ws_t m ->
-  Stack unit
-  (requires fun h -> live h ws)
-  (ensures  fun h0 _ h1 -> modifies (loc ws) h0 h1 /\
-    as_seq h1 ws == V.transpose_ws (as_seq h0 ws))
-
 let transpose_ws #m ws =
   match lanes m with
   | 1 -> ()
   | 4 -> transpose_ws4 ws
 
-inline_for_extraction noextract
-val load_ws: #a:keccak_alg -> #m:m_spec{is_supported m}
-  -> b:multibuf (lanes m) 256ul
-  -> ws:ws_t m ->
-  Stack unit
-  (requires fun h -> live_multi h b /\ live h ws /\ disjoint_multi b ws)
-  (ensures  fun h0 _ h1 -> modifies (loc ws) h0 h1 /\
-    as_seq h1 ws == V.load_ws #a #m (as_seq_multi h0 b))
-
 let load_ws #a #m b ws =
   load_blocks #a #m b ws;
   transpose_ws ws
 
-inline_for_extraction noextract
-val loadState: #a:keccak_alg -> #m:m_spec{is_supported m}
-  -> rateInBytes:size_t{v rateInBytes > 0 /\ v rateInBytes <= 200}
-  -> b:multibuf (lanes m) 256ul
-  -> s:state_t m ->
-  Stack unit
-  (requires fun h -> live_multi h b /\ live h s /\ disjoint_multi b s /\
-    (forall l. l < lanes m ==> (forall i. (i >= v rateInBytes /\ i < 256) ==>
-      Seq.index (as_seq_multi h b).(|l|) i == u8 0)))
-  (ensures  fun h0 _ h1 -> modifies (loc s) h0 h1 /\
-    as_seq h1 s == V.loadState #a #m (v rateInBytes) (as_seq_multi h0 b) (as_seq h0 s))
-
-let loadState #a #m _ b s =
+let loadState #a #m rateInBytes b s =
   let init_h0 = ST.get() in
   push_frame ();
+  let h0_f = ST.get() in
   let ws = create 32ul (zero_element m) in
   let h0 = ST.get() in
   Lib.NTuple.eq_intro (as_seq_multi h0 b) (as_seq_multi init_h0 b);
@@ -642,16 +387,12 @@ let loadState #a #m _ b s =
   (fun i ->
     Lib.LoopCombinators.unfold_repeati 25 (V.loadState_inner m (as_seq h1 ws)) (as_seq h1 s) (v i);
     s.(i) <- s.(i) ^| ws.(i));
-  pop_frame()
-
-inline_for_extraction noextract
-val transpose_s_ws4:
-    #m:m_spec{lanes m == 4}
-  -> ws:ws_t m
-  -> Stack unit
-    (requires fun h -> live h ws)
-    (ensures  fun h0 _ h1 -> modifies (loc ws) h0 h1 /\
-      as_seq h1 ws == V.transpose_s_ws (as_seq h0 ws))
+  let h1_f = ST.get() in
+  pop_frame();
+  let h1 = ST.get() in
+  fresh_frame_modifies init_h0 h0_f;
+  popped_modifies h1_f h1;
+  modifies_remove_fresh_frame init_h0 h0_f h1 (loc s)
 
 let transpose_s_ws4 #m ws =
   let (ws0,ws1,ws2,ws3) =
@@ -673,27 +414,10 @@ let transpose_s_ws4 #m ws =
   create32 ws ws0 ws4 ws8 ws12 ws16 ws20 ws24 ws28 ws1 ws5 ws9 ws13 ws17 ws21 ws25
     ws29 ws2 ws6 ws10 ws14 ws18 ws22 ws26 ws30 ws3 ws7 ws11 ws15 ws19 ws23 ws27 ws31
 
-inline_for_extraction noextract
-val transpose_s_ws: #m:m_spec{is_supported m} -> ws:ws_t m ->
-  Stack unit
-  (requires fun h -> live h ws)
-  (ensures  fun h0 _ h1 -> modifies (loc ws) h0 h1 /\
-    as_seq h1 ws == V.transpose_s_ws (as_seq h0 ws))
-
 let transpose_s_ws #m ws =
   match lanes m with
   | 1 -> ()
   | 4 -> transpose_s_ws4 ws
-
-inline_for_extraction noextract
-val storeState: #a:keccak_alg -> #m:m_spec{is_supported m}
-  -> s:state_t m
-  -> hbuf:lbuffer uint8 (size (lanes m) *! 32ul *! 8ul) ->
-  Stack unit
-  (requires fun h -> live h hbuf /\ live h s /\ disjoint hbuf s /\
-    as_seq h hbuf == LSeq.create (lanes m * 32 * word_length a) (u8 0))
-  (ensures  fun h0 _ h1 -> modifies (loc hbuf) h0 h1 /\
-    as_seq h1 hbuf == V.storeState #a #m (as_seq h0 s))
 
 let storeState #a #m s hbuf =
   push_frame ();
@@ -703,28 +427,8 @@ let storeState #a #m s hbuf =
   Lib.IntVector.Serialize.vecs_store_le hbuf ws;
   pop_frame()
 
-inline_for_extraction noextract
-val next_blocks:
-  rateInBytes:size_t{v rateInBytes > 0 /\ v rateInBytes <= 200}
-  -> nextBlock:lbuffer uint8 256ul ->
-  Stack unit
-  (requires fun h -> live h nextBlock /\
-    as_seq h nextBlock == LSeq.create 256 (u8 0))
-  (ensures  fun h0 _ h1 -> modifies (loc nextBlock) h0 h1 /\
-    as_seq h1 nextBlock == V.next_blocks (v rateInBytes) (as_seq h0 nextBlock))
-
 let next_blocks rateInBytes nextBlock =
   nextBlock.(rateInBytes -! 1ul) <- u8 0x80
-
-inline_for_extraction noextract
-val next_block1: #m:m_spec{lanes m == 1}
-  -> rateInBytes:size_t{v rateInBytes > 0 /\ v rateInBytes <= 200}
-  -> b:multibuf (lanes m) 256ul ->
-  Stack unit
-  (requires fun h -> live_multi h b /\
-    as_seq_multi h b == next_block_seq_zero m)
-  (ensures  fun h0 _ h1 -> modifies_multi b h0 h1 /\
-    as_seq_multi h1 b == V.next_block #m (v rateInBytes) (as_seq_multi h0 b))
 
 let next_block1 #m rateInBytes b =
   let h0 = ST.get() in
@@ -733,16 +437,6 @@ let next_block1 #m rateInBytes b =
   let h1 = ST.get() in
   Lib.NTuple.eq_intro (as_seq_multi h1 b) 
     (V.next_block1 #m (v rateInBytes) (as_seq_multi h0 b))
-
-inline_for_extraction noextract
-val next_block4: #m:m_spec{lanes m == 4}
-  -> rateInBytes:size_t{v rateInBytes > 0 /\ v rateInBytes <= 200}
-  -> b:multibuf (lanes m) 256ul ->
-  Stack unit
-  (requires fun h -> live_multi h b /\ internally_disjoint b /\ 
-    as_seq_multi h b == next_block_seq_zero m)
-  (ensures  fun h0 _ h1 -> modifies_multi b h0 h1 /\
-    as_seq_multi h1 b == V.next_block #m (v rateInBytes) (as_seq_multi h0 b))
 
 let next_block4 #m rateInBytes b =
   let h0 = ST.get() in
@@ -757,28 +451,10 @@ let next_block4 #m rateInBytes b =
   Lib.NTuple.eq_intro (as_seq_multi h1 b) 
     (V.next_block4 #m (v rateInBytes) (as_seq_multi h0 b))
 
-inline_for_extraction noextract
-val next_block: #m:m_spec{is_supported m}
-  -> rateInBytes:size_t{v rateInBytes > 0 /\ v rateInBytes <= 200}
-  -> b:multibuf (lanes m) 256ul ->
-  Stack unit
-  (requires fun h -> live_multi h b /\ internally_disjoint b /\ 
-    as_seq_multi h b == next_block_seq_zero m)
-  (ensures  fun h0 _ h1 -> modifies_multi b h0 h1 /\
-    as_seq_multi h1 b == V.next_block #m (v rateInBytes) (as_seq_multi h0 b))
-
 let next_block #m rateInBytes b =
   match lanes m with
   | 1 -> next_block1 #m rateInBytes b
   | 4 -> next_block4 #m rateInBytes b
-
-inline_for_extraction noextract
-val alloc_multi1: m:m_spec{lanes m == 1} ->
-  StackInline (multibuf (lanes m) 256ul)
-  (requires fun h -> True)
-  (ensures  fun h0 b h1 -> live_multi h1 b /\
-    stack_allocated_multi b h0 h1 (Seq.create 256 (u8 0)) /\
-    as_seq_multi h1 b == next_block_seq_zero m)
 
 let alloc_multi1 m =
   let b = create 256ul (u8 0) in
@@ -786,14 +462,6 @@ let alloc_multi1 m =
   let h0 = ST.get() in
   Lib.NTuple.eq_intro (as_seq_multi h0 b) (next_block_seq_zero m);
   b
-
-inline_for_extraction noextract
-val alloc_multi4: m:m_spec{lanes m == 4} ->
-  StackInline (multibuf (lanes m) 256ul)
-  (requires fun h -> True)
-  (ensures  fun h0 b h1 -> live_multi h1 b /\ internally_disjoint b /\
-    stack_allocated_multi b h0 h1 (Seq.create 256 (u8 0)) /\
-    as_seq_multi h1 b == next_block_seq_zero m)
 
 let alloc_multi4 m =
   let b0 = create 256ul (u8 0) in
@@ -805,27 +473,10 @@ let alloc_multi4 m =
   Lib.NTuple.eq_intro (as_seq_multi h0 b) (next_block_seq_zero m);
   b
 
-inline_for_extraction noextract
-val alloc_multi: m:m_spec{is_supported m} ->
-  StackInline (multibuf (lanes m) 256ul)
-  (requires fun h -> True)
-  (ensures  fun h0 b h1 -> live_multi h1 b /\ internally_disjoint b /\
-    stack_allocated_multi b h0 h1 (Seq.create 256 (u8 0)) /\
-    as_seq_multi h1 b == next_block_seq_zero m)
-
 let alloc_multi m =
   match lanes m with
   | 1 -> alloc_multi1 m
   | 4 -> alloc_multi4 m
-
-inline_for_extraction noextract
-val absorb_next: #a:keccak_alg -> #m:m_spec{is_supported m}
-  -> rateInBytes:size_t{v rateInBytes > 0 /\ v rateInBytes <= 200}
-  -> s:state_t m ->
-  Stack unit
-  (requires fun h -> live h s)
-  (ensures  fun h0 _ h1 -> modifies (loc s) h0 h1 /\
-    as_seq h1 s == V.absorb_next #a #m (v rateInBytes) (as_seq h0 s))
 
 let absorb_next #a #m rateInBytes s =
   push_frame ();
@@ -839,35 +490,8 @@ let absorb_next #a #m rateInBytes s =
   state_permute m s;
   pop_frame()
 
-inline_for_extraction noextract
-val load_last_blocks:
-  rateInBytes:size_t{v rateInBytes > 0 /\ v rateInBytes <= 200}
-  -> rem:size_t{v rem < v rateInBytes}
-  -> delimitedSuffix:byte_t
-  -> lastBlock:lbuffer uint8 256ul ->
-  Stack unit
-  (requires fun h -> live h lastBlock /\ (forall i. (i >= v rem /\ i < 256) ==>
-    Seq.index (as_seq h lastBlock) i == u8 0))
-  (ensures  fun h0 _ h1 -> modifies (loc lastBlock) h0 h1 /\
-    as_seq h1 lastBlock ==
-      V.load_last_blocks (v rateInBytes) (v rem) delimitedSuffix (as_seq h0 lastBlock))
-
 let load_last_blocks _ rem delimitedSuffix lastBlock =
   lastBlock.(rem) <- byte_to_uint8 delimitedSuffix
-
-inline_for_extraction noextract
-val load_last_block1: #m:m_spec{lanes m == 1}
-  -> rateInBytes:size_t{v rateInBytes > 0 /\ v rateInBytes <= 200}
-  -> rem:size_t{v rem < v rateInBytes}
-  -> delimitedSuffix:byte_t
-  -> b:multibuf (lanes m) 256ul ->
-  Stack unit
-  (requires fun h -> live_multi h b /\
-    (forall l. l < lanes m ==> (forall i. (i >= v rem /\ i < 256) ==>
-      Seq.index (as_seq_multi h b).(|l|) i == u8 0)))
-  (ensures  fun h0 _ h1 -> modifies_multi b h0 h1 /\
-    as_seq_multi h1 b ==
-      V.load_last_block #m (v rateInBytes) (v rem) delimitedSuffix (as_seq_multi h0 b))
 
 let load_last_block1 #m rateInBytes rem delimitedSuffix b =
   let h0 = ST.get() in
@@ -876,20 +500,6 @@ let load_last_block1 #m rateInBytes rem delimitedSuffix b =
   let h1 = ST.get() in
   Lib.NTuple.eq_intro (as_seq_multi h1 b) 
     (V.load_last_block #m (v rateInBytes) (v rem) delimitedSuffix (as_seq_multi h0 b))
-
-inline_for_extraction noextract
-val load_last_block4: #m:m_spec{lanes m == 4}
-  -> rateInBytes:size_t{v rateInBytes > 0 /\ v rateInBytes <= 200}
-  -> rem:size_t{v rem < v rateInBytes}
-  -> delimitedSuffix:byte_t
-  -> b:multibuf (lanes m) 256ul ->
-  Stack unit
-  (requires fun h -> live_multi h b /\ internally_disjoint b /\
-    (forall l. l < lanes m ==> (forall i. (i >= v rem /\ i < 256) ==>
-      Seq.index (as_seq_multi h b).(|l|) i == u8 0)))
-  (ensures  fun h0 _ h1 -> modifies_multi b h0 h1 /\
-    as_seq_multi h1 b ==
-      V.load_last_block #m (v rateInBytes) (v rem) delimitedSuffix (as_seq_multi h0 b))
 
 let load_last_block4 #m rateInBytes rem delimitedSuffix b =
   let h0 = ST.get() in
@@ -904,38 +514,10 @@ let load_last_block4 #m rateInBytes rem delimitedSuffix b =
   Lib.NTuple.eq_intro (as_seq_multi h1 b) 
     (V.load_last_block #m (v rateInBytes) (v rem) delimitedSuffix (as_seq_multi h0 b))
 
-inline_for_extraction noextract
-val load_last_block: #m:m_spec{is_supported m}
-  -> rateInBytes:size_t{v rateInBytes > 0 /\ v rateInBytes <= 200}
-  -> rem:size_t{v rem < v rateInBytes}
-  -> delimitedSuffix:byte_t
-  -> b:multibuf (lanes m) 256ul ->
-  Stack unit
-  (requires fun h -> live_multi h b /\ internally_disjoint b /\
-    (forall l. l < lanes m ==> (forall i. (i >= v rem /\ i < 256) ==>
-      Seq.index (as_seq_multi h b).(|l|) i == u8 0)))
-  (ensures  fun h0 _ h1 -> modifies_multi b h0 h1 /\
-    as_seq_multi h1 b ==
-      V.load_last_block #m (v rateInBytes) (v rem) delimitedSuffix (as_seq_multi h0 b))
-
 let load_last_block #m rateInBytes rem delimitedSuffix b =
   match lanes m with
   | 1 -> load_last_block1 #m rateInBytes rem delimitedSuffix b
   | 4 -> load_last_block4 #m rateInBytes rem delimitedSuffix b
-
-inline_for_extraction noextract
-val absorb_last: #a:keccak_alg -> #m:m_spec{is_supported m}
-  -> rateInBytes:size_t{v rateInBytes > 0 /\ v rateInBytes <= 200}
-  -> rem:size_t{v rem < v rateInBytes}
-  -> delimitedSuffix:byte_t
-  -> b:multibuf (lanes m) 256ul
-  -> s:state_t m ->
-  Stack unit
-  (requires fun h -> live_multi h b /\ live h s /\ disjoint_multi b s /\ internally_disjoint b /\
-    (forall l. l < lanes m ==> (forall i. (i >= v rem /\ i < 256) ==>
-      Seq.index (as_seq_multi h b).(|l|) i == u8 0)))
-  (ensures  fun h0 _ h1 -> modifies (loc s |+| loc_multi b) h0 h1 /\
-    as_seq h1 s == V.absorb_last #a #m delimitedSuffix (v rateInBytes) (v rem) (as_seq_multi h0 b) (as_seq h0 s))
 
 let absorb_last #a #m rateInBytes rem delimitedSuffix b s =
   logand_spec delimitedSuffix (byte 0x80);
@@ -955,44 +537,13 @@ let absorb_last #a #m rateInBytes rem delimitedSuffix b s =
        (rem =. (rateInBytes -! 1ul)) then state_permute m s;
   absorb_next #a #m rateInBytes s
 
-inline_for_extraction noextract
-val absorb_inner: #a:keccak_alg -> #m:m_spec{is_supported m}
-  -> rateInBytes:size_t{v rateInBytes > 0 /\ v rateInBytes <= 200}
-  -> b:multibuf (lanes m) 256ul
-  -> s:state_t m ->
-  Stack unit
-  (requires fun h -> live_multi h b /\ live h s /\ disjoint_multi b s /\
-    (forall l. l < lanes m ==> (forall i. (i >= v rateInBytes /\ i < 256) ==>
-      Seq.index (as_seq_multi h b).(|l|) i == u8 0)))
-  (ensures  fun h0 _ h1 -> modifies (loc s) h0 h1 /\
-    as_seq h1 s == V.absorb_inner #a #m (v rateInBytes) (as_seq_multi h0 b) (as_seq h0 s))
-
 let absorb_inner #a #m rateInBytes b s =
   loadState #a #m rateInBytes b s;
   state_permute m s
 
-noextract
-let preserves_disjoint_multi #lanes #len #len' (b:multibuf lanes len) (r:multibuf lanes len') =
-    (forall a l (x:lbuffer a l). disjoint_multi b x ==> disjoint_multi r x)
-
-inline_for_extraction noextract
-let get_multiblock_t (m:m_spec{is_supported m}) =
-    rateInBytes:size_t{v rateInBytes > 0 /\ v rateInBytes <= 200}
-  -> len:size_t
-  -> b:multibuf (lanes m) len
-  -> i:size_t{v i < v len / v rateInBytes}
-  -> b':multibuf (lanes m) 256ul ->
-  Stack unit
-  (requires fun h -> live_multi h b /\ live_multi h b' /\
-    internally_disjoint b' /\ disjoint_multi_multi b b' /\
-    as_seq_multi h b' == next_block_seq_zero m)
-  (ensures  fun h0 _ h1 -> modifies_multi b' h0 h1 /\
-    as_seq_multi h1 b' == V.get_multiblock_spec (v rateInBytes) (v len) (as_seq_multi h0 b) (v i))
-
-inline_for_extraction noextract
-val get_multiblock_1: #m:m_spec{lanes m == 1} -> get_multiblock_t m
 let get_multiblock_1 #m rateInBytes len b i b' =
   let h0 = ST.get() in
+  assert (v (i *! rateInBytes) == v i * v rateInBytes);
   assert (v i * v rateInBytes < v len);
   assert (v i + 1 <= v len / v rateInBytes);
   assert ((v i + 1) * v rateInBytes <= v len);
@@ -1004,11 +555,10 @@ let get_multiblock_1 #m rateInBytes len b i b' =
   let h1 = ST.get() in
   Lib.NTuple.eq_intro (as_seq_multi h1 b') (V.get_multiblock_spec #m (v rateInBytes) (v len) (as_seq_multi h0 b) (v i))
 
-#push-options "--z3rlimit 400"
-inline_for_extraction noextract
-val get_multiblock_4: #m:m_spec{lanes m == 4} -> get_multiblock_t m
+#push-options "--max_ifuel 1 --max_fuel 1"
 let get_multiblock_4 #m rateInBytes len b i b' =
   let h0 = ST.get() in
+  assert (v (i *! rateInBytes) == v i * v rateInBytes);
   assert (v i * v rateInBytes < v len);
   assert (v i + 1 <= v len / v rateInBytes);
   assert ((v i + 1) * v rateInBytes <= v len);
@@ -1017,6 +567,7 @@ let get_multiblock_4 #m rateInBytes len b i b' =
   let (bl0,(bl1,(bl2,bl3))) = tup4 b' in
   assert (internally_disjoint4 bl0 bl1 bl2 bl3);
   assert (disjoint4_4 b0 b1 b2 b3 bl0 bl1 bl2 bl3);
+  loc_multi4 b;
   update_sub bl0 0ul rateInBytes (sub b0 (i *! rateInBytes) rateInBytes);
   update_sub bl1 0ul rateInBytes (sub b1 (i *! rateInBytes) rateInBytes);
   update_sub bl2 0ul rateInBytes (sub b2 (i *! rateInBytes) rateInBytes);
@@ -1026,52 +577,18 @@ let get_multiblock_4 #m rateInBytes len b i b' =
   Lib.NTuple.eq_intro (as_seq_multi h1 b') (V.get_multiblock_spec #m (v rateInBytes) (v len) (as_seq_multi h0 b) (v i))
 #pop-options
 
-inline_for_extraction noextract
-val get_multiblock: #m:m_spec{is_supported m} -> get_multiblock_t m
 let get_multiblock #m rateInBytes len b i b' =
   match lanes m with
   | 1 -> get_multiblock_1 #m rateInBytes len b i b'
   | 4 -> get_multiblock_4 #m rateInBytes len b i b'
 
-#push-options "--max_ifuel 1"
-inline_for_extraction noextract
-val get_multilast_disjoint_helper: rateInBytes:size_t{v rateInBytes > 0 /\ v rateInBytes <= 200}
-  -> len:size_t
-  -> b:lbuffer uint8 len
-  -> b':lbuffer uint8 256ul ->
-  Stack unit
-  (requires fun h -> live h b /\ live h b' /\ disjoint b' b)
-  (ensures  fun h0 _ h1 -> modifies loc_none h0 h1 /\ (
-    let rem = len %. rateInBytes in
-    let b0 = gsub b (len -! rem) rem in
-    disjoint b' b0))
-let get_multilast_disjoint_helper rateInBytes len b b' =
-  let rem = len %. rateInBytes in
-  let b0 = sub b (len -! rem) rem in
-  assert (disjoint b' b0)
-#pop-options
-
-inline_for_extraction noextract
-let get_multilast_t (m:m_spec{is_supported m}) =
-    rateInBytes:size_t{v rateInBytes > 0 /\ v rateInBytes <= 200}
-  -> len:size_t
-  -> b:multibuf (lanes m) len
-  -> b':multibuf (lanes m) 256ul ->
-  Stack unit
-  (requires fun h -> live_multi h b /\ live_multi h b' /\
-    internally_disjoint b' /\ disjoint_multi_multi b b' /\
-    as_seq_multi h b' == next_block_seq_zero m)
-  (ensures  fun h0 _ h1 -> modifies_multi b' h0 h1 /\
-    as_seq_multi h1 b' == V.get_multilast_spec (v rateInBytes) (v len) (as_seq_multi h0 b))
-
-#push-options "--max_ifuel 1 --z3rlimit 200"
-inline_for_extraction noextract
-val get_multilast_1: #m:m_spec{lanes m == 1} -> get_multilast_t m
 let get_multilast_1 #m rateInBytes len b b' =
   let h0 = ST.get() in
   Lib.NTuple.eq_intro (as_seq_multi h0 b') (next_block_seq_zero m);
   let rem = len %. rateInBytes in
   assert (v (len %. rateInBytes) == v len % v rateInBytes);
+  Math.Lemmas.lemma_mod_lt (v len) (v rateInBytes);
+  assert (v rem <= v len);
   assert (v (len -! rem) == v len - v rem);
   let b0 = tup1 b in
   let bl0 = tup1 b' in
@@ -1079,25 +596,20 @@ let get_multilast_1 #m rateInBytes len b b' =
   update_sub bl0 0ul rem (sub b0 (len -! rem) rem);
   let h1 = ST.get() in
   Lib.NTuple.eq_intro (as_seq_multi h1 b') (V.get_multilast_spec #m (v rateInBytes) (v len) (as_seq_multi h0 b))
-#pop-options
 
-#push-options "--max_ifuel 1 --z3rlimit 500"
-inline_for_extraction noextract
-val get_multilast_4: #m:m_spec{lanes m == 4} -> get_multilast_t m
+#push-options "--max_ifuel 1"
 let get_multilast_4 #m rateInBytes len b b' =
   let h0 = ST.get() in
   Lib.NTuple.eq_intro (as_seq_multi h0 b') (next_block_seq_zero m);
   let rem = len %. rateInBytes in
   assert (v (len %. rateInBytes) == v len % v rateInBytes);
+  Math.Lemmas.lemma_mod_lt (v len) (v rateInBytes);
+  assert (v rem <= v len);
   assert (v (len -! rem) == v len - v rem);
   let (b0,(b1,(b2,b3))) = tup4 b in
   let (bl0,(bl1,(bl2,bl3))) = tup4 b' in
   assert (internally_disjoint4 bl0 bl1 bl2 bl3);
   assert (disjoint4_4 b0 b1 b2 b3 bl0 bl1 bl2 bl3);
-  get_multilast_disjoint_helper rateInBytes len b0 bl0;
-  get_multilast_disjoint_helper rateInBytes len b1 bl1;
-  get_multilast_disjoint_helper rateInBytes len b2 bl2;
-  get_multilast_disjoint_helper rateInBytes len b3 bl3;
   let h0' = ST.get() in
   Lib.NTuple.eq_intro (as_seq_multi h0' b) (as_seq_multi h0 b);
   Lib.NTuple.eq_intro (as_seq_multi h0' b') (next_block_seq_zero m);
@@ -1110,28 +622,15 @@ let get_multilast_4 #m rateInBytes len b b' =
   Lib.NTuple.eq_intro (as_seq_multi h1 b') (V.get_multilast_spec #m (v rateInBytes) (v len) (as_seq_multi h0 b))
 #pop-options
 
-inline_for_extraction noextract
-val get_multilast: #m:m_spec{is_supported m} -> get_multilast_t m
 let get_multilast #m rateInBytes len b b' =
   match lanes m with
   | 1 -> get_multilast_1 #m rateInBytes len b b'
   | 4 -> get_multilast_4 #m rateInBytes len b b'
 
-inline_for_extraction noextract
-val absorb_inner_block: #a:keccak_alg -> #m:m_spec{is_supported m}
-  -> rateInBytes:size_t{v rateInBytes > 0 /\ v rateInBytes <= 200}
-  -> len:size_t
-  -> b:multibuf (lanes m) len
-  -> i:size_t{v i < v len / v rateInBytes}
-  -> s:state_t m ->
-  Stack unit
-  (requires fun h -> live_multi h b /\ live h s /\ disjoint_multi b s)
-  (ensures  fun h0 _ h1 -> modifies (loc s) h0 h1 /\
-    as_seq h1 s == V.absorb_inner_block #a #m (v rateInBytes) (v len) (as_seq_multi h0 b) (v i) (as_seq h0 s))
-
 let absorb_inner_block #a #m rateInBytes len b i s =
   let h0 = ST.get() in
   push_frame ();
+  let h0_f = ST.get() in
   if (lanes m = 1) then loc_multi1 b else loc_multi4 b;
   let b' = alloc_multi m in
   let h0' = ST.get() in
@@ -1142,23 +641,19 @@ let absorb_inner_block #a #m rateInBytes len b i s =
   assert (forall l. l < lanes m ==> (forall j. (j >= v rateInBytes /\ j < 256) ==>
     Seq.index (as_seq_multi h0' b').(|l|) j == u8 0));
   absorb_inner #a #m rateInBytes b' s;
-  let h1 = ST.get() in
-  assert (modifies (loc s |+| loc_multi b') h0 h1);
+  let h1_f = ST.get() in
+  LSeq.eq_intro (as_seq h1_f s)
+    (V.absorb_inner_block #a #m (v rateInBytes) (v len) (as_seq_multi h0 b) (v i) (as_seq h0 s));
   pop_frame ();
   let h1 = ST.get() in
-  LSeq.eq_intro (as_seq h1 s)
-    (V.absorb_inner_block #a #m (v rateInBytes) (v len) (as_seq_multi h0 b) (v i) (as_seq h0 s))
-
-inline_for_extraction noextract
-val absorb_inner_nblocks: #a:keccak_alg -> #m:m_spec{is_supported m}
-  -> rateInBytes:size_t{v rateInBytes > 0 /\ v rateInBytes <= 200}
-  -> len:size_t
-  -> b:multibuf (lanes m) len
-  -> s:state_t m ->
-  Stack unit
-  (requires fun h -> live_multi h b /\ live h s /\ disjoint_multi b s)
-  (ensures  fun h0 _ h1 -> modifies (loc s) h0 h1 /\
-    as_seq h1 s == V.absorb_inner_nblocks #a #m (v rateInBytes) (v len) (as_seq_multi h0 b) (as_seq h0 s))
+  LSeq.eq_intro (as_seq h1 s) (as_seq h1_f s);
+  fresh_frame_modifies h0 h0_f;
+  popped_modifies h1_f h1;
+  modifies_remove_fresh_frame h0 h0_f h1 (loc s);
+  assert (modifies (loc s) h0 h1);
+  assert (modifies (loc s) h0 h1 /\
+    as_seq h1 s ==
+      V.absorb_inner_block #a #m (v rateInBytes) (v len) (as_seq_multi h0 b) (v i) (as_seq h0 s))
 
 let absorb_inner_nblocks #a #m rateInBytes len b s =
   let h0 = ST.get() in
@@ -1170,104 +665,77 @@ let absorb_inner_nblocks #a #m rateInBytes len b s =
     Lib.NTuple.eq_intro (as_seq_multi h0' b) (as_seq_multi h0 b);
     absorb_inner_block #a #m rateInBytes len b i s)
 
-inline_for_extraction noextract
-val absorb_final: #a:keccak_alg -> #m:m_spec{is_supported m}
-  -> rateInBytes:size_t{v rateInBytes > 0 /\ v rateInBytes <= 200}
-  -> len:size_t
-  -> b:multibuf (lanes m) len
-  -> delimitedSuffix:byte_t
-  -> s:state_t m ->
-  Stack unit
-  (requires fun h -> live_multi h b /\ live h s /\ disjoint_multi b s)
-  (ensures  fun h0 _ h1 -> modifies (loc s) h0 h1 /\
-    as_seq h1 s ==
-      V.absorb_final #a #m (as_seq h0 s) (v rateInBytes) (v len) (as_seq_multi h0 b) delimitedSuffix)
+let absorb_final_get #a #m rateInBytes len b b' delimitedSuffix s =
+  if (lanes m = 1) then loc_multi1 b' else loc_multi4 b';
+  assert (v (len %. rateInBytes) == v len % v rateInBytes);
+  get_multilast #m rateInBytes len b b';
+  absorb_last #a #m rateInBytes (len %. rateInBytes) delimitedSuffix b' s
 
-#push-options "--max_ifuel 1 --z3rlimit 200"
 let absorb_final #a #m rateInBytes len b delimitedSuffix s =
   let h0 = ST.get() in
   assert (v (len %. rateInBytes) == v len % v rateInBytes);
-  let rem = len %. rateInBytes in
+  Math.Lemmas.lemma_mod_lt (v len) (v rateInBytes);
   push_frame ();
+  let h0_f = ST.get() in
   if (lanes m = 1) then loc_multi1 b else loc_multi4 b;
   let b' = alloc_multi m in
   let h0' = ST.get() in
   Lib.NTuple.eq_intro (as_seq_multi h0' b) (as_seq_multi h0 b);
-  get_multilast #m rateInBytes len b b';
   if (lanes m = 1) then loc_multi1 b' else loc_multi4 b';
-  let h0' = ST.get() in
-  assert (modifies_multi b' h0 h0');
-  absorb_last #a #m rateInBytes rem delimitedSuffix b' s;
-  let h1 = ST.get() in
-  assert (modifies (loc s |+| loc_multi b') h0 h1);
+  absorb_final_get #a #m rateInBytes len b b' delimitedSuffix s;
+  let h1_f = ST.get() in
+  assert (as_seq h1_f s ==
+    V.absorb_final #a #m (as_seq h0 s) (v rateInBytes) (v len) (as_seq_multi h0 b) delimitedSuffix);
   pop_frame ();
   let h1 = ST.get() in
-  LSeq.eq_intro (as_seq h1 s)
-    (V.absorb_final #a #m (as_seq h0 s) (v rateInBytes) (v len) (as_seq_multi h0 b) delimitedSuffix);
-  ()
-#pop-options
-
-inline_for_extraction noextract
-val absorb: #a:keccak_alg -> #m:m_spec{is_supported m}
-  -> rateInBytes:size_t{v rateInBytes > 0 /\ v rateInBytes <= 200}
-  -> len:size_t
-  -> b:multibuf (lanes m) len
-  -> delimitedSuffix:byte_t
-  -> s:state_t m ->
-  Stack unit
-  (requires fun h -> live_multi h b /\ live h s /\ disjoint_multi b s)
-  (ensures  fun h0 _ h1 -> modifies (loc s) h0 h1 /\
-    as_seq h1 s == V.absorb #a #m (as_seq h0 s) (v rateInBytes) (v len) (as_seq_multi h0 b) delimitedSuffix)
+  assert (as_seq h1 s == as_seq h1_f s);
+  fresh_frame_modifies h0 h0_f;
+  popped_modifies h1_f h1;
+  modifies_remove_fresh_frame h0 h0_f h1 (loc s);
+  assert (modifies (loc s) h0 h1);
+  assert (modifies (loc s) h0 h1 /\
+    as_seq h1 s ==
+      V.absorb_final #a #m (as_seq h0 s) (v rateInBytes) (v len) (as_seq_multi h0 b) delimitedSuffix)
 
 let absorb #a #m rateInBytes len b delimitedSuffix s =
+  let h0 = ST.get() in
   if (lanes m = 1) then loc_multi1 b else loc_multi4 b;
   absorb_inner_nblocks #a #m rateInBytes len b s;
-  absorb_final #a #m rateInBytes len b delimitedSuffix s
+  absorb_final #a #m rateInBytes len b delimitedSuffix s;
+  let h1 = ST.get() in
+  assert (as_seq h1 s ==
+    V.absorb #a #m (as_seq h0 s) (v rateInBytes) (v len) (as_seq_multi h0 b) delimitedSuffix);
+  assert (modifies (loc s) h0 h1 /\ as_seq h1 s ==
+    V.absorb #a #m (as_seq h0 s) (v rateInBytes) (v len) (as_seq_multi h0 b) delimitedSuffix)
 
-inline_for_extraction noextract
-val update_output1:
-  #m:m_spec{lanes m == 1}
-  -> block:lbuffer uint8 (size (lanes m) *! 256ul)
-  -> rateInBytes:size_t{v rateInBytes > 0 /\ v rateInBytes <= 200}
-  -> outputByteLen:size_t
-  -> i:size_t{v i < v outputByteLen / v rateInBytes}
-  -> b:multibuf (lanes m) outputByteLen ->
-  Stack unit
-  (requires fun h -> live h block /\ live_multi h b /\ internally_disjoint b /\
-    disjoint_multi b block)
-  (ensures  fun h0 _ h1 -> modifies_multi b h0 h1 /\ as_seq_multi h1 b ==
-      V.update_b #m (as_seq h0 block) (v rateInBytes) (v outputByteLen) (v i) (as_seq_multi h0 b))
-
+#push-options "--z3rlimit 200"
 let update_output1 #m block rateInBytes outputByteLen i b =
   let h0 = ST.get() in
+  loc_multi1 b;
+  let b0 = tup1 b in
+  assert (disjoint b0 block);
+  assert (v (i *! rateInBytes) == v i * v rateInBytes);
   assert (v i * v rateInBytes < v outputByteLen);
   assert (v i + 1 <= v outputByteLen / v rateInBytes);
   assert ((v i + 1) * v rateInBytes <= v outputByteLen);
   assert (v i * v rateInBytes + v rateInBytes <= v outputByteLen);
-  update_sub b.(|0|) (i *! rateInBytes) rateInBytes (sub block 0ul rateInBytes);
+  update_sub b0 (i *! rateInBytes) rateInBytes (sub block 0ul rateInBytes);
   let h1 = ST.get() in
   Lib.NTuple.eq_intro (as_seq_multi h1 b)
     (V.update_b #m (as_seq h0 block) (v rateInBytes) (v outputByteLen) (v i) (as_seq_multi h0 b))
+#pop-options
 
-inline_for_extraction noextract
-val update_output4:
-  #m:m_spec{lanes m == 4}
-  -> block:lbuffer uint8 (size (lanes m) *! 256ul)
-  -> rateInBytes:size_t{v rateInBytes > 0 /\ v rateInBytes <= 200}
-  -> outputByteLen:size_t
-  -> i:size_t{v i < v outputByteLen / v rateInBytes}
-  -> b:multibuf (lanes m) outputByteLen ->
-  Stack unit
-  (requires fun h -> live h block /\ live_multi h b /\ internally_disjoint b /\
-    disjoint_multi b block)
-  (ensures  fun h0 _ h1 -> modifies_multi b h0 h1 /\ as_seq_multi h1 b ==
-      V.update_b #m (as_seq h0 block) (v rateInBytes) (v outputByteLen) (v i) (as_seq_multi h0 b))
-
+#push-options "--z3rlimit 200"
 let update_output4 #m block rateInBytes outputByteLen i b =
   let h0 = ST.get() in
   loc_multi4 b;
   let (b0,(b1,(b2,b3))) = tup4 b in
   assert (internally_disjoint4 b0 b1 b2 b3);
+  assert (disjoint b0 block);
+  assert (disjoint b1 block);
+  assert (disjoint b2 block);
+  assert (disjoint b3 block);
+  assert (v (i *! rateInBytes) == v i * v rateInBytes);
   assert (v i * v rateInBytes < v outputByteLen);
   assert (v i + 1 <= v outputByteLen / v rateInBytes);
   assert ((v i + 1) * v rateInBytes <= v outputByteLen);
@@ -1279,39 +747,12 @@ let update_output4 #m block rateInBytes outputByteLen i b =
   let h1 = ST.get() in
   Lib.NTuple.eq_intro (as_seq_multi h1 b)
     (V.update_b #m (as_seq h0 block) (v rateInBytes) (v outputByteLen) (v i) (as_seq_multi h0 b))
-
-inline_for_extraction noextract
-val update_output:
-  #m:m_spec{is_supported m}
-  -> block:lbuffer uint8 (size (lanes m) *! 256ul)
-  -> rateInBytes:size_t{v rateInBytes > 0 /\ v rateInBytes <= 200}
-  -> outputByteLen:size_t
-  -> i:size_t{v i < v outputByteLen / v rateInBytes}
-  -> b:multibuf (lanes m) outputByteLen ->
-  Stack unit
-  (requires fun h -> live h block /\ live_multi h b /\ internally_disjoint b /\
-    disjoint_multi b block)
-  (ensures  fun h0 _ h1 -> modifies_multi b h0 h1 /\ as_seq_multi h1 b ==
-      V.update_b #m (as_seq h0 block) (v rateInBytes) (v outputByteLen) (v i) (as_seq_multi h0 b))
+#pop-options
 
 let update_output #m block rateInBytes outputByteLen i b =
   match lanes m with
   | 1 -> update_output1 #m block rateInBytes outputByteLen i b
   | 4 -> update_output4 #m block rateInBytes outputByteLen i b
-
-inline_for_extraction noextract
-val update_output_last1:
-  #m:m_spec{lanes m == 1}
-  -> block:lbuffer uint8 (size (lanes m) *! 256ul)
-  -> rateInBytes:size_t{v rateInBytes > 0 /\ v rateInBytes <= 200}
-  -> outputByteLen:size_t
-  -> outRem:size_t{v outRem == v outputByteLen % v rateInBytes}
-  -> b:multibuf (lanes m) outputByteLen ->
-  Stack unit
-  (requires fun h -> live h block /\ live_multi h b /\ internally_disjoint b /\
-    disjoint_multi b block)
-  (ensures  fun h0 _ h1 -> modifies_multi b h0 h1 /\ as_seq_multi h1 b ==
-      V.update_b_last #m (as_seq h0 block) (v rateInBytes) (v outputByteLen) (v outRem) (as_seq_multi h0 b))
 
 let update_output_last1 #m block rateInBytes outputByteLen outRem b =
   let h0 = ST.get() in
@@ -1320,20 +761,6 @@ let update_output_last1 #m block rateInBytes outputByteLen outRem b =
   let h1 = ST.get() in
   Lib.NTuple.eq_intro (as_seq_multi h1 b)
     (V.update_b_last #m (as_seq h0 block) (v rateInBytes) (v outputByteLen) (v outRem) (as_seq_multi h0 b))
-
-inline_for_extraction noextract
-val update_output_last4:
-  #m:m_spec{lanes m == 4}
-  -> block:lbuffer uint8 (size (lanes m) *! 256ul)
-  -> rateInBytes:size_t{v rateInBytes > 0 /\ v rateInBytes <= 200}
-  -> outputByteLen:size_t
-  -> outRem:size_t{v outRem == v outputByteLen % v rateInBytes}
-  -> b:multibuf (lanes m) outputByteLen ->
-  Stack unit
-  (requires fun h -> live h block /\ live_multi h b /\ internally_disjoint b /\
-    disjoint_multi b block)
-  (ensures  fun h0 _ h1 -> modifies_multi b h0 h1 /\ as_seq_multi h1 b ==
-      V.update_b_last #m (as_seq h0 block) (v rateInBytes) (v outputByteLen) (v outRem) (as_seq_multi h0 b))
 
 let update_output_last4 #m block rateInBytes outputByteLen outRem b =
   let h0 = ST.get() in
@@ -1349,40 +776,10 @@ let update_output_last4 #m block rateInBytes outputByteLen outRem b =
   Lib.NTuple.eq_intro (as_seq_multi h1 b)
     (V.update_b_last #m (as_seq h0 block) (v rateInBytes) (v outputByteLen) (v outRem) (as_seq_multi h0 b))
 
-inline_for_extraction noextract
-val update_output_last:
-  #m:m_spec{is_supported m}
-  -> block:lbuffer uint8 (size (lanes m) *! 256ul)
-  -> rateInBytes:size_t{v rateInBytes > 0 /\ v rateInBytes <= 200}
-  -> outputByteLen:size_t
-  -> outRem:size_t{v outRem == v outputByteLen % v rateInBytes}
-  -> b:multibuf (lanes m) outputByteLen ->
-  Stack unit
-  (requires fun h -> live h block /\ live_multi h b /\ internally_disjoint b /\
-    disjoint_multi b block)
-  (ensures  fun h0 _ h1 -> modifies_multi b h0 h1 /\ as_seq_multi h1 b ==
-      V.update_b_last #m (as_seq h0 block) (v rateInBytes) (v outputByteLen) (v outRem) (as_seq_multi h0 b))
-
 let update_output_last #m block rateInBytes outputByteLen outRem b =
   match lanes m with
   | 1 -> update_output_last1 #m block rateInBytes outputByteLen outRem b
   | 4 -> update_output_last4 #m block rateInBytes outputByteLen outRem b
-
-inline_for_extraction noextract
-val squeeze_inner: #a:keccak_alg -> #m:m_spec{is_supported m}
-  -> rateInBytes:size_t{v rateInBytes > 0 /\ v rateInBytes <= 200}
-  -> outputByteLen:size_t
-  -> i:size_t{v i < v outputByteLen / v rateInBytes}
-  -> s:state_t m
-  -> b:multibuf (lanes m) outputByteLen ->
-  Stack unit
-  (requires fun h -> live_multi h b /\ live h s /\ internally_disjoint b /\
-    disjoint_multi b s)
-  (ensures  fun h0 _ h1 -> modifies (loc s |+| loc_multi b) h0 h1 /\
-    (let s', b' = 
-      V.squeeze_inner #a #m (v rateInBytes) (v outputByteLen) (v i) (as_seq h0 s, as_seq_multi h0 b) in
-      as_seq h1 s == s' /\
-      as_seq_multi h1 b == b'))
 
 let squeeze_inner #a #m rateInBytes outputByteLen i s b =
   let h0 = ST.get() in
@@ -1401,22 +798,6 @@ let squeeze_inner #a #m rateInBytes outputByteLen i s b =
   LSeq.eq_intro (as_seq h1 s) s';
   Lib.NTuple.eq_intro (as_seq_multi h1 b) b'
 
-inline_for_extraction noextract
-val squeeze_nblocks:# a:keccak_alg -> #m:m_spec{is_supported m}
-  -> s:state_t m
-  -> rateInBytes:size_t{v rateInBytes > 0 /\ v rateInBytes <= 200}
-  -> outputByteLen:size_t
-  -> b:multibuf (lanes m) outputByteLen ->
-  Stack unit
-    (requires fun h -> live_multi h b /\ live h s /\ internally_disjoint b /\
-      disjoint_multi b s)
-    (ensures  fun h0 _ h1 ->
-      modifies (loc s |+| loc_multi b) h0 h1 /\
-      (let s', b' = 
-        V.squeeze_nblocks #a #m (v rateInBytes) (v outputByteLen) (as_seq h0 s, as_seq_multi h0 b) in
-        as_seq h1 s == s' /\
-        as_seq_multi h1 b == b'))
-
 let squeeze_nblocks #a #m s rateInBytes outputByteLen b =
   [@ inline_let]
   let refl h i : GTot ((V.state_spec m) & (V.multiseq (lanes m) (v outputByteLen))) = as_seq h s, as_seq_multi h b in
@@ -1433,21 +814,9 @@ let squeeze_nblocks #a #m s rateInBytes outputByteLen b =
     squeeze_inner #a #m rateInBytes outputByteLen i s b
   )
 
-inline_for_extraction noextract
-val squeeze_last:# a:keccak_alg -> #m:m_spec{is_supported m}
-  -> s:state_t m
-  -> rateInBytes:size_t{v rateInBytes > 0 /\ v rateInBytes <= 200}
-  -> outputByteLen:size_t
-  -> b:multibuf (lanes m) outputByteLen ->
-  Stack unit
-    (requires fun h -> live_multi h b /\ live h s /\ internally_disjoint b /\
-      disjoint_multi b s)
-    (ensures  fun h0 _ h1 ->
-      modifies_multi b h0 h1 /\
-      as_seq_multi h1 b == V.squeeze_last #a #m (as_seq h0 s) (v rateInBytes) (v outputByteLen) (as_seq_multi h0 b))
-
 let squeeze_last #a #m s rateInBytes outputByteLen b =
   let h0 = ST.get () in
+  assert (v (outputByteLen %. rateInBytes) == v outputByteLen % v rateInBytes);
   push_frame();
   let remOut = outputByteLen %. rateInBytes in
   let hbuf = create (size (lanes m) *. 32ul *. 8ul) (u8 0) in
@@ -1459,50 +828,38 @@ let squeeze_last #a #m s rateInBytes outputByteLen b =
   let h1 = ST.get() in
   Lib.NTuple.eq_intro (as_seq_multi h1 b) (V.squeeze_last #a #m (as_seq h0 s) (v rateInBytes) (v outputByteLen) (as_seq_multi h0 b))
 
-inline_for_extraction noextract
-val squeeze:# a:keccak_alg -> #m:m_spec{is_supported m}
-  -> s:state_t m
-  -> rateInBytes:size_t{v rateInBytes > 0 /\ v rateInBytes <= 200}
-  -> outputByteLen:size_t
-  -> b:multibuf (lanes m) outputByteLen ->
-  Stack unit
-    (requires fun h -> live_multi h b /\ live h s /\ internally_disjoint b /\
-      disjoint_multi b s)
-    (ensures  fun h0 _ h1 ->
-      modifies (loc s |+| loc_multi b) h0 h1 /\
-      as_seq_multi h1 b == V.squeeze #a #m (as_seq h0 s) (v rateInBytes) (v outputByteLen) (as_seq_multi h0 b))
-
 let squeeze #a #m s rateInBytes outputByteLen b =
   squeeze_nblocks #a #m s rateInBytes outputByteLen b;
   squeeze_last #a #m s rateInBytes outputByteLen b
 
-inline_for_extraction noextract
-val keccak:# a:keccak_alg -> #m:m_spec{is_supported m}
-  -> rate:size_t{v rate % 8 == 0 /\ v rate / 8 > 0 /\ v rate <= 1600}
-  -> inputByteLen:size_t
-  -> input:multibuf (lanes m) inputByteLen
-  -> delimitedSuffix:byte_t
-  -> outputByteLen:size_t
-  -> output:multibuf (lanes m) outputByteLen ->
-  Stack unit
-    (requires fun h -> live_multi h input /\ live_multi h output /\
-      internally_disjoint output /\ disjoint_multi_multi input output)
-    (ensures  fun h0 _ h1 ->
-      modifies_multi output h0 h1 /\
-      as_seq_multi h1 output ==
-        V.keccak #a #m (v rate) (v inputByteLen) (as_seq_multi h0 input) delimitedSuffix (v outputByteLen) (as_seq_multi h0 output))
+let keccak_get #a #m rate inputByteLen input delimitedSuffix outputByteLen output s =
+  let h0 = ST.get () in
+  assert (v (rate /. 8ul) == v rate / 8);
+  let rateInBytes = rate /. 8ul in
+  absorb #a #m rateInBytes inputByteLen input delimitedSuffix s;
+  let h0' = ST.get () in
+  Lib.NTuple.eq_intro (as_seq_multi h0' output) (as_seq_multi h0 output);
+  squeeze #a #m s rateInBytes outputByteLen output
 
 let keccak #a #m rate inputByteLen input delimitedSuffix outputByteLen output =
   let h0 = ST.get () in
+  assert (v (rate /. 8ul) == v rate / 8);
+  if (lanes m = 1) then loc_multi1 output else loc_multi4 output;
   push_frame();
+  let h0_f = ST.get() in
   let rateInBytes = rate /. 8ul in
   let s = create 25ul (zero_element m) in
   let h0' = ST.get () in
   Lib.NTuple.eq_intro (as_seq_multi h0' input) (as_seq_multi h0 input);
-  absorb #a #m rateInBytes inputByteLen input delimitedSuffix s;
-  let h0' = ST.get () in
   Lib.NTuple.eq_intro (as_seq_multi h0' output) (as_seq_multi h0 output);
-  squeeze #a #m s rateInBytes outputByteLen output;
+  keccak_get #a #m rate inputByteLen input delimitedSuffix outputByteLen output s;
+  let h1_f = ST.get() in
+  assert (as_seq_multi h1_f output ==
+    V.keccak #a #m (v rate) (v inputByteLen) (as_seq_multi h0 input) delimitedSuffix
+    (v outputByteLen) (as_seq_multi h0 output));
   pop_frame();
   let h1 = ST.get() in
-  Lib.NTuple.eq_intro (as_seq_multi h1 output) (V.keccak #a #m (v rate) (v inputByteLen) (as_seq_multi h0 input) delimitedSuffix (v outputByteLen) (as_seq_multi h0 output))
+  Lib.NTuple.eq_intro (as_seq_multi h1 output) (as_seq_multi h1_f output);
+  fresh_frame_modifies h0 h0_f;
+  popped_modifies h1_f h1;
+  modifies_remove_fresh_frame h0 h0_f h1 (loc_multi output)
