code/sha3/Hacl.Spec.SHA3.Equiv.fsti
@@ -1,0 +1,811 @@
+module Hacl.Spec.SHA3.Equiv
+
+open FStar.Mul
+open Lib.IntTypes
+open Lib.NTuple
+open Lib.Sequence
+open Lib.IntVector
+open Lib.LoopCombinators
+
+open Spec.Hash.Definitions
+open Hacl.Spec.SHA3.Vec
+open Hacl.Spec.SHA3.Vec.Common
+module Spec = Spec.SHA3
+module BSeq = Lib.ByteSequence
+
+#set-options "--z3rlimit 50 --fuel 0 --ifuel 0"
+
+(* state_theta0 *)
+
+val state_theta_inner_C_lemma_l:
+  m:m_spec
+  -> s:state_spec m
+  -> i:size_nat{i < 5}
+  -> _C:lseq (element_t m) 5
+  -> l:nat{l < lanes m} ->
+  Lemma
+   ((_C_v (state_theta_inner_C m s i _C)).[l] ==
+    Spec.state_theta_inner_C (state_spec_v s).[l] i (_C_v _C).[l])
+
+val state_theta0_loop:
+  m:m_spec
+  -> s:state_spec m
+  -> _C:lseq (element_t m) 5
+  -> l:nat{l < lanes m}
+  -> n:nat{n <= 5} ->
+  Lemma
+   ((_C_v (repeati n (state_theta_inner_C m s) _C)).[l] ==
+    repeati n (Spec.state_theta_inner_C (state_spec_v s).[l]) (_C_v _C).[l])
+
+val state_theta0_lemma_l:
+  m:m_spec
+  -> s:state_spec m
+  -> _C:lseq (element_t m) 5
+  -> l:nat{l < lanes m} ->
+  Lemma ((_C_v (state_theta0 m s _C)).[l] == Spec.state_theta0 (state_spec_v s).[l] (_C_v _C).[l])
+
+(* state_theta1 *)
+
+val state_theta_inner_s_inner_lemma_l:
+  m:m_spec
+  -> x:index
+  -> _D:element_t m
+  -> y:index
+  -> s:state_spec m
+  -> l:nat{l < lanes m} ->
+  Lemma
+   ((state_spec_v (state_theta_inner_s_inner m x _D y s)).[l] ==
+    Spec.state_theta_inner_s_inner x (vec_v _D).[l] y (state_spec_v s).[l])
+
+val state_theta_inner_s_loop:
+  m:m_spec
+  -> _C:lseq (element_t m) 5
+  -> x:index
+  -> s:state_spec m
+  -> l:nat{l < lanes m}
+  -> n:nat{n <= 5} ->
+  Lemma
+   (let _D_u64 = ((_C_v _C).[l]).[(x + 4) % 5] ^. (Spec.rotl ((_C_v _C).[l]).[(x + 1) % 5] (size 1)) in
+    let _D_elem = _C.[(x + 4) % 5] ^| (_C.[(x + 1) % 5] <<<| (size 1)) in
+    (state_spec_v (repeati n (state_theta_inner_s_inner m x _D_elem) s)).[l] ==
+    repeati n (Spec.state_theta_inner_s_inner x _D_u64) (state_spec_v s).[l])
+
+val state_theta_inner_s_lemma_l:
+  m:m_spec
+  -> _C:lseq (element_t m) 5
+  -> x:index
+  -> s:state_spec m
+  -> l:nat{l < lanes m} ->
+  Lemma ((state_spec_v (state_theta_inner_s m _C x s)).[l] ==
+         Spec.state_theta_inner_s (_C_v _C).[l] x (state_spec_v s).[l])
+
+val state_theta1_loop:
+  m:m_spec
+  -> _C:lseq (element_t m) 5
+  -> s:state_spec m
+  -> l:nat{l < lanes m}
+  -> n:nat{n <= 5} ->
+  Lemma
+   ((state_spec_v (repeati n (state_theta_inner_s m _C) s)).[l] ==
+    repeati n (Spec.state_theta_inner_s (_C_v _C).[l]) (state_spec_v s).[l])
+
+val state_theta1_lemma_l:
+  m:m_spec
+  -> _C:lseq (element_t m) 5
+  -> s:state_spec m
+  -> l:nat{l < lanes m} ->
+  Lemma ((state_spec_v (state_theta1 m _C s)).[l] ==
+         Spec.state_theta1 (_C_v _C).[l] (state_spec_v s).[l])
+
+(* state_theta *)
+
+val state_theta_lemma_l:
+  m:m_spec
+  -> s:state_spec m
+  -> l:nat{l < lanes m} ->
+  Lemma ((state_spec_v (state_theta m s)).[l] ==
+         Spec.state_theta (state_spec_v s).[l])
+
+(* state_pi_rho *)
+
+val state_pi_rho_inner_lemma_l:
+  m:m_spec
+  -> i:size_nat{i < 24}
+  -> current:element_t m
+  -> s:state_spec m
+  -> l:nat{l < lanes m} ->
+  Lemma
+   (let c', s' = state_pi_rho_inner m i (current, s) in
+    (((vec_v c').[l] <: uint64), (state_spec_v s').[l]) ==
+    Spec.state_pi_rho_inner i ((vec_v current).[l], (state_spec_v s).[l]))
+
+val state_pi_rho_loop:
+  m:m_spec
+  -> s:state_spec m
+  -> l:nat{l < lanes m}
+  -> n:nat{n <= 24} ->
+  Lemma
+    (let c_elem = get m s 1 0 in
+     let c_u64 = Spec.get (state_spec_v s).[l] 1 0 in
+     let c', s' = repeat_gen n (state_pi_rho_s m)
+       (state_pi_rho_inner m) (c_elem, s) in
+     let c'_s, s'_s = repeat_gen n Spec.state_pi_rho_s
+       Spec.state_pi_rho_inner (c_u64, (state_spec_v s).[l]) in
+     (vec_v c').[l] == c'_s /\ (state_spec_v s').[l] == s'_s)
+
+val state_pi_rho_lemma_l:
+  m:m_spec
+  -> s:state_spec m
+  -> l:nat{l < lanes m} ->
+  Lemma ((state_spec_v (state_pi_rho m s)).[l] ==
+           Spec.state_pi_rho (state_spec_v s).[l])
+
+(* state_chi *)
+
+val state_chi_inner0_lemma_l:
+  m:m_spec
+  -> s_pi_rho:state_spec m
+  -> y:index
+  -> x:index
+  -> s:state_spec m
+  -> l:nat{l < lanes m} ->
+  Lemma
+   ((state_spec_v (state_chi_inner0 m s_pi_rho y x s)).[l] ==
+      Spec.state_chi_inner0 (state_spec_v s_pi_rho).[l] y x (state_spec_v s).[l])
+
+val state_chi_inner1_loop:
+  m:m_spec
+  -> s_pi_rho:state_spec m
+  -> y:index
+  -> s:state_spec m
+  -> l:nat{l < lanes m}
+  -> n:nat{n <= 5} ->
+  Lemma
+   ((state_spec_v (repeati n (state_chi_inner0 m s_pi_rho y) s)).[l] ==
+      repeati n (Spec.state_chi_inner0 (state_spec_v s_pi_rho).[l] y) (state_spec_v s).[l])
+
+val state_chi_inner1_lemma_l:
+  m:m_spec
+  -> s_pi_rho:state_spec m
+  -> y:index
+  -> s:state_spec m
+  -> l:nat{l < lanes m} ->
+  Lemma ((state_spec_v (state_chi_inner1 m s_pi_rho y s)).[l] ==
+         Spec.state_chi_inner1 (state_spec_v s_pi_rho).[l] y (state_spec_v s).[l])
+
+val state_chi_loop:
+  m:m_spec
+  -> s_pi_rho:state_spec m
+  -> s:state_spec m
+  -> l:nat{l < lanes m}
+  -> n:nat{n <= 5} ->
+  Lemma
+   ((state_spec_v (repeati n (state_chi_inner1 m s_pi_rho) s)).[l] ==
+      repeati n (Spec.state_chi_inner1 (state_spec_v s_pi_rho).[l]) (state_spec_v s).[l])
+
+val state_chi_lemma_l:
+  m:m_spec
+  -> s_pi_rho:state_spec m
+  -> l:nat{l < lanes m} ->
+  Lemma ((state_spec_v (state_chi m s_pi_rho)).[l] ==
+           Spec.state_chi (state_spec_v s_pi_rho).[l])
+
+(* state_iota *)
+
+val state_iota_lemma_l:
+  m:m_spec
+  -> s:state_spec m
+  -> round:size_nat{round < 24}
+  -> l:nat{l < lanes m} ->
+  Lemma
+   ((state_spec_v (state_iota m s round)).[l] ==
+      Spec.state_iota (state_spec_v s).[l] round)
+
+(* state_permute *)
+
+val state_permute1_lemma_l:
+  m:m_spec
+  -> round:size_nat{round < 24}
+  -> s:state_spec m
+  -> l:nat{l < lanes m} ->
+  Lemma ((state_spec_v (state_permute1 m round s)).[l] ==
+         Spec.state_permute1 round (state_spec_v s).[l])
+
+val state_permute_loop:
+  m:m_spec
+  -> s:state_spec m
+  -> l:nat{l < lanes m}
+  -> n:nat{n <= 24} ->
+  Lemma
+   ((state_spec_v (repeati n (state_permute1 m) s)).[l] ==
+      repeati n Spec.state_permute1 (state_spec_v s).[l])
+
+val state_permute_lemma_l:
+  m:m_spec
+  -> s:state_spec m
+  -> l:nat{l < lanes m} ->
+  Lemma ((state_spec_v (state_permute m s)).[l] ==
+           Spec.state_permute (state_spec_v s).[l])
+
+(* loadState *)
+
+val load_blocks_lemma_ij:
+    #a:keccak_alg
+  -> #m:m_spec
+  -> b:multiblock_spec a m
+  -> j:nat{j < lanes m}
+  -> i:nat{i < 32} ->
+  Lemma (let l = lanes m in
+    let ind = (i / l * l + j) * word_length a in
+    (vec_v (load_blocks b).[i]).[j] ==
+    BSeq.uint_from_bytes_le
+      (Seq.slice b.(|i % l|) ind (ind + word_length a)))
+
+val load_blocks_lemma_ij_subst:
+    #a:keccak_alg
+  -> #m:m_spec
+  -> b:multiblock_spec a m
+  -> j:nat{j < lanes m}
+  -> i:nat{i < 32} ->
+  Lemma (let l = lanes m in
+    (vec_v (load_blocks b).[i / l * l + j]).[i % l] ==
+    BSeq.uint_from_bytes_le
+      (Seq.slice b.(|j|) (i * word_length a) (i * word_length a + word_length a)))
+
+val load_ws_lemma_l:
+    #a:keccak_alg
+  -> #m:m_spec{is_supported m}
+  -> b:multiblock_spec a m
+  -> l:nat{l < lanes m}
+  -> i:nat{i < 25} ->
+  Lemma ((ws_spec_v (load_ws b)).[l].[i] == BSeq.uint_from_bytes_le
+      (Seq.slice (Seq.slice b.(|l|) 0 200) (i * word_length a) (i * word_length a + word_length a)))
+
+val loadState_inner_lemma_l:
+    #a:keccak_alg
+  -> #m:m_spec{is_supported m}
+  -> b:multiblock_spec a m
+  -> s:state_spec m
+  -> l:nat{l < lanes m}
+  -> i:nat{i < 25} ->
+  Lemma ((state_spec_v (loadState_inner m (load_ws b) i s)).[l] ==
+    Spec.loadState_inner (Seq.slice b.(|l|) 0 200) i (state_spec_v s).[l])
+
+val loadState_loop_full:
+  #a:keccak_alg
+  -> #m:m_spec{is_supported m}
+  -> r:size_nat{r > 0 /\ r <= 200}
+  -> b:multiblock_spec a m
+  -> s:state_spec m
+  -> l:nat{l < lanes m}
+  -> n:nat{n <= 25} ->
+  Lemma
+  ((state_spec_v (repeati n (loadState_inner m (load_ws b)) s)).[l] ==
+    repeati n (Spec.loadState_inner (Seq.slice b.(|l|) 0 200))
+      (state_spec_v s).[l])
+
+val update_sub_b_lemma:
+    #a:keccak_alg
+  -> #m:m_spec{is_supported m}
+  -> r:size_nat{r > 0 /\ r <= 200}
+  -> b:multiblock_spec a m
+  -> l:nat{l < lanes m} ->
+  Lemma
+  (requires
+    forall l. l < lanes m ==> (forall j. (j >= r /\ j < 256) ==> Seq.index b.(|l|) j == u8 0))
+  (ensures
+    Seq.slice b.(|l|) 0 200 == update_sub (create 200 (u8 0)) 0 r (Seq.slice b.(|l|) 0 r))
+
+val loadState_loop:
+    #a:keccak_alg
+  -> #m:m_spec{is_supported m}
+  -> r:size_nat{r > 0 /\ r <= 200}
+  -> b:multiblock_spec a m
+  -> s:state_spec m
+  -> l:nat{l < lanes m}
+  -> n:nat{n <= 25} ->
+  Lemma
+  (requires
+    forall l. l < lanes m ==> (forall j. (j >= r /\ j < 256) ==> Seq.index b.(|l|) j == u8 0))
+  (ensures (let bs = update_sub (create 200 (u8 0)) 0 r (Seq.slice b.(|l|) 0 r) in
+    (state_spec_v (repeati n (loadState_inner m (load_ws b)) s)).[l] ==
+      repeati n (Spec.loadState_inner bs) (state_spec_v s).[l]))
+
+val loadState_lemma_l:
+  #a:keccak_alg
+  -> #m:m_spec{is_supported m}
+  -> r:size_nat{r > 0 /\ r <= 200}
+  -> b:multiblock_spec a m
+  -> s:state_spec m
+  -> l:nat{l < lanes m} ->
+  Lemma
+  (requires
+    forall l. l < lanes m ==> (forall j. (j >= r /\ j < 256) ==> Seq.index b.(|l|) j == u8 0))
+  (ensures 
+    (state_spec_v (loadState #a #m r b s)).[l] ==
+      Spec.loadState r (Seq.slice b.(|l|) 0 r) (state_spec_v s).[l])
+
+(* storeState *)
+
+val storeState_lemma_ij:
+    #a:keccak_alg
+  -> #m:m_spec{is_supported m}
+  -> s:state_spec m
+  -> j:nat{j < lanes m}
+  -> i:nat{i < 25 * word_length a} ->
+  Lemma
+   ((storeState #a #m s).[j * (32 * word_length a) + i] ==
+      (BSeq.uint_to_bytes_le (Seq.index (state_spec_v s).[j] (i / word_length a))).[i % word_length a])
+
+val storeState_lemma_ij_sub:
+    #a:keccak_alg
+  -> #m:m_spec{is_supported m}
+  -> s:state_spec m
+  -> j:nat{j < lanes m}
+  -> i:nat{i < 25} ->
+  Lemma
+   (sub (sub (storeState #a #m s) (j * (32 * word_length a)) (25 * word_length a)) (i * word_length a) (word_length a) ==
+      BSeq.uint_to_bytes_le (Seq.index (state_spec_v s).[j] i))
+
+let storeState_inner_unroll (s:Spec.state) : Tot (BSeq.lbytes 200) =
+  let block = Spec.storeState_inner s 0 (create 200 (u8 0)) in
+  let block = Spec.storeState_inner s 1 block in
+  let block = Spec.storeState_inner s 2 block in
+  let block = Spec.storeState_inner s 3 block in
+  let block = Spec.storeState_inner s 4 block in
+  let block = Spec.storeState_inner s 5 block in
+  let block = Spec.storeState_inner s 6 block in
+  let block = Spec.storeState_inner s 7 block in
+  let block = Spec.storeState_inner s 8 block in
+  let block = Spec.storeState_inner s 9 block in
+  let block = Spec.storeState_inner s 10 block in
+  let block = Spec.storeState_inner s 11 block in
+  let block = Spec.storeState_inner s 12 block in
+  let block = Spec.storeState_inner s 13 block in
+  let block = Spec.storeState_inner s 14 block in
+  let block = Spec.storeState_inner s 15 block in
+  let block = Spec.storeState_inner s 16 block in
+  let block = Spec.storeState_inner s 17 block in
+  let block = Spec.storeState_inner s 18 block in
+  let block = Spec.storeState_inner s 19 block in
+  let block = Spec.storeState_inner s 20 block in
+  let block = Spec.storeState_inner s 21 block in
+  let block = Spec.storeState_inner s 22 block in
+  let block = Spec.storeState_inner s 23 block in
+  let block = Spec.storeState_inner s 24 block in
+  block
+
+val storeState_inner_loop:
+  s:Spec.state  ->
+  Lemma
+   (storeState_inner_unroll s ==
+      repeati 25 (Spec.storeState_inner s) (create 200 (u8 0)))
+
+val storeState_inner_unroll_sub_0_6:
+    #a:keccak_alg
+  -> #m:m_spec{is_supported m}
+  -> s:Spec.state
+  -> i:nat{i < 6} ->
+  Lemma
+   (sub (storeState_inner_unroll s) (i * 8) 8 ==
+      BSeq.uint_to_bytes_le #U64 s.[i])
+
+val storeState_inner_unroll_sub_6_12:
+    #a:keccak_alg
+  -> #m:m_spec{is_supported m}
+  -> s:Spec.state
+  -> i:nat{i >= 6 /\ i < 12} ->
+  Lemma
+   (sub (storeState_inner_unroll s) (i * 8) 8 ==
+      BSeq.uint_to_bytes_le #U64 s.[i])
+
+val storeState_inner_unroll_sub_12_18:
+    #a:keccak_alg
+  -> #m:m_spec{is_supported m}
+  -> s:Spec.state
+  -> i:nat{i >= 12 /\ i < 18} ->
+  Lemma
+   (sub (storeState_inner_unroll s) (i * 8) 8 ==
+      BSeq.uint_to_bytes_le #U64 s.[i])
+
+val storeState_inner_unroll_sub_18_25:
+    #a:keccak_alg
+  -> #m:m_spec{is_supported m}
+  -> s:Spec.state
+  -> i:nat{i >= 18 /\ i < 25} ->
+  Lemma
+   (sub (storeState_inner_unroll s) (i * 8) 8 ==
+      BSeq.uint_to_bytes_le #U64 s.[i])
+
+val storeState_inner_unroll_sub:
+    #a:keccak_alg
+  -> #m:m_spec{is_supported m}
+  -> s:Spec.state
+  -> i:nat{i < 25} ->
+  Lemma
+   (sub (storeState_inner_unroll s) (i * 8) 8 ==
+      BSeq.uint_to_bytes_le #U64 s.[i])
+
+val sub_word_length_lemma:
+    #a:keccak_alg
+  -> l0:lseq uint8 (25 * word_length a)
+  -> l1:lseq uint8 (25 * word_length a) ->
+  Lemma
+  (requires
+    forall (i:nat{0 <= i /\ i < 25}).
+    (forall (j:nat{0 <= j /\ j < word_length a}).
+      Seq.index (sub l0 (i*word_length a) (word_length a)) j ==
+        Seq.index (sub l1 (i*word_length a) (word_length a)) j))
+  (ensures l0 == l1)
+
+val storeState_lemma_l:
+  #a:keccak_alg
+  -> #m:m_spec{is_supported m}
+  -> r:size_nat{r <= 200}
+  -> s:state_spec m
+  -> l:nat{l < lanes m} ->
+  Lemma
+   (sub (storeState #a #m s) (l * (32 * word_length a)) r ==
+     Spec.storeState r (state_spec_v s).[l])
+
+val storeState_update_b_lemma_l:
+  #a:keccak_alg
+  -> #m:m_spec{is_supported m}
+  -> r:size_nat{r > 0 /\ r <= 200}
+  -> outputByteLen:size_nat
+  -> i:size_nat{i < outputByteLen / r}
+  -> b:multiseq (lanes m) outputByteLen
+  -> s:state_spec m
+  -> l:nat{l < lanes m} ->
+  Lemma
+   (let block = storeState #a #m s in
+    let b' = update_b #m block r outputByteLen i b in
+    i * r + r <= outputByteLen /\
+    sub #uint8 #outputByteLen b'.(|l|) (i * r) r ==
+     Spec.storeState r (state_spec_v s).[l] /\
+    (forall j. (j < i * r /\ j >= i * r + r) ==>
+      Seq.index b'.(|l|) j == Seq.index b.(|l|) j))
+
+val storeState_update_b_last_lemma_l:
+  #a:keccak_alg
+  -> #m:m_spec{is_supported m}
+  -> r:size_nat{r > 0 /\ r <= 200}
+  -> outputByteLen:size_nat
+  -> outRem:size_nat{outRem == outputByteLen % r}
+  -> b:multiseq (lanes m) outputByteLen
+  -> s:state_spec m
+  -> l:nat{l < lanes m} ->
+  Lemma
+   (let block = storeState #a #m s in
+    let b' = update_b_last #m block r outputByteLen outRem b in
+    outRem <= outputByteLen /\
+    sub #uint8 #outputByteLen b'.(|l|) (outputByteLen - outRem) outRem ==
+     Spec.storeState outRem (state_spec_v s).[l] /\
+    (forall i. (i < outputByteLen - outRem) ==>
+      Seq.index b'.(|l|) i == Seq.index b.(|l|) i))
+
+(* absorb_inner *)
+
+val absorb_inner_lemma_l:
+  #a:keccak_alg
+  -> #m:m_spec{is_supported m}
+  -> r:size_nat{r > 0 /\ r <= 200}
+  -> input:multiseq (lanes m) 256{forall l. l < lanes m ==> 
+     (forall i. (i >= r /\ i < 256) ==> Seq.index input.(|l|) i == u8 0)}
+  -> s:state_spec m
+  -> l:nat{l < lanes m} ->
+  Lemma
+   ((state_spec_v (absorb_inner #a #m r input s)).[l] ==
+    Spec.absorb_inner r (sub #uint8 #256 input.(|l|) 0 r) (state_spec_v s).[l])
+
+(* absorb_inner_block *)
+
+val absorb_inner_block_lemma_l:
+  #a:keccak_alg
+  -> #m:m_spec{is_supported m}
+  -> r:size_nat{r > 0 /\ r <= 200}
+  -> inputByteLen:nat
+  -> input:multiseq (lanes m) inputByteLen
+  -> i:nat{i < inputByteLen / r}
+  -> s:state_spec m
+  -> l:nat{l < lanes m} ->
+  Lemma
+   ((state_spec_v (absorb_inner_block #a #m r inputByteLen input i s)).[l] ==
+    repeat_blocks_f r input.(|l|) (Spec.absorb_inner r) (inputByteLen / r) i (state_spec_v s).[l])
+
+(* absorb_inner_nblocks *)
+
+val absorb_inner_loop:
+  #a:keccak_alg
+  -> #m:m_spec{is_supported m}
+  -> r:size_nat{r > 0 /\ r <= 200}
+  -> inputByteLen:nat
+  -> input:multiseq (lanes m) inputByteLen
+  -> s:state_spec m
+  -> l:nat{l < lanes m}
+  -> n:nat{n <= inputByteLen / r} ->
+  Lemma
+   ((state_spec_v (repeati n (absorb_inner_block #a #m r inputByteLen input) s)).[l] ==
+    repeati n (repeat_blocks_f r input.(|l|) (Spec.absorb_inner r) (inputByteLen / r)) (state_spec_v s).[l])
+
+val absorb_inner_nblocks_lemma_l:
+  #a:keccak_alg
+  -> #m:m_spec{is_supported m}
+  -> r:size_nat{r > 0 /\ r <= 200}
+  -> inputByteLen:nat
+  -> input:multiseq (lanes m) inputByteLen
+  -> s:state_spec m
+  -> l:nat{l < lanes m} ->
+  Lemma
+   ((state_spec_v (absorb_inner_nblocks #a #m r inputByteLen input s)).[l] ==
+    repeati (inputByteLen / r) (repeat_blocks_f r input.(|l|) (Spec.absorb_inner r) (inputByteLen / r)) (state_spec_v s).[l])
+
+(* absorb_next *)
+
+val next_block_lemma_l:
+  #m:m_spec{is_supported m}
+  -> r:size_nat{r > 0 /\ r <= 200}
+  -> l:nat{l < lanes m} ->
+  Lemma
+   (sub #uint8 #256 ((next_block #m r (next_block_seq_zero m)).(|l|)) 0 r ==
+    ((create r (u8 0)).[r - 1] <- u8 0x80))
+
+val absorb_next_lemma_l:
+  #a:keccak_alg
+  -> #m:m_spec{is_supported m}
+  -> r:size_nat{r > 0 /\ r <= 200}
+  -> s:state_spec m
+  -> l:nat{l < lanes m} ->
+  Lemma
+   ((state_spec_v (absorb_next #a #m r s)).[l] ==
+    Spec.absorb_next (state_spec_v s).[l] r)
+
+(* absorb_last *)
+
+val load_last_block_lemma_helper:
+  #m:m_spec{is_supported m}
+  -> delimitedSuffix:byte_t
+  -> r:size_nat{r > 0 /\ r <= 200}
+  -> rem:size_nat{rem < r}
+  -> input:BSeq.lbytes rem ->
+  Lemma(let b_0 = update_sub (create r (u8 0)) 0 rem input in
+        let b = b_0.[rem] <- byte_to_uint8 delimitedSuffix in
+        (forall i. (i >= 0 /\ i < rem) ==> Seq.index b i == Seq.index input i) /\
+        Seq.index b rem == byte_to_uint8 delimitedSuffix /\
+        (forall i. (i >= (rem + 1) /\ i < r) ==> Seq.index b i == u8 0))
+
+val load_last_block_lemma_l:
+  #m:m_spec{is_supported m}
+  -> delimitedSuffix:byte_t
+  -> r:size_nat{r > 0 /\ r <= 200}
+  -> rem:size_nat{rem < r}
+  -> input:multiseq (lanes m) 256{forall l. l < lanes m ==> 
+       (forall i. (i >= rem /\ i < 256) ==> Seq.index input.(|l|) i == u8 0)}
+  -> l:nat{l < lanes m} ->
+  Lemma
+   (let b = update_sub (create r (u8 0)) 0 rem (sub #uint8 #256 input.(|l|) 0 rem) in
+    sub #uint8 #256 ((load_last_block #m r rem delimitedSuffix input).(|l|)) 0 r ==
+      (b.[rem] <- byte_to_uint8 delimitedSuffix))
+
+val absorb_last_lemma_l:
+  #a:keccak_alg
+  -> #m:m_spec{is_supported m}
+  -> delimitedSuffix:byte_t
+  -> r:size_nat{r > 0 /\ r <= 200}
+  -> rem:size_nat{rem < r}
+  -> input:multiseq (lanes m) 256{forall l. l < lanes m ==> 
+       (forall i. (i >= rem /\ i < 256) ==> Seq.index input.(|l|) i == u8 0)}
+  -> s:state_spec m
+  -> l:nat{l < lanes m} ->
+  Lemma
+   ((state_spec_v (absorb_last #a #m delimitedSuffix r rem input s)).[l] ==
+    Spec.absorb_last delimitedSuffix r rem (sub #uint8 #256 input.(|l|) 0 rem) (state_spec_v s).[l])
+
+(* absorb_final *)
+
+val absorb_final_lemma_l:
+  #a:keccak_alg
+  -> #m:m_spec{is_supported m}
+  -> delimitedSuffix:byte_t
+  -> r:size_nat{r > 0 /\ r <= 200}
+  -> inputByteLen:nat
+  -> input:multiseq (lanes m) inputByteLen
+  -> s:state_spec m
+  -> l:nat{l < lanes m} ->
+  Lemma
+   (inputByteLen - (inputByteLen / r) * r <= inputByteLen /\
+   (inputByteLen / r) * r == inputByteLen - (inputByteLen % r) /\
+    (state_spec_v (absorb_final #a #m s r inputByteLen input delimitedSuffix)).[l] ==
+      Spec.absorb_last delimitedSuffix r (inputByteLen % r)
+        (Seq.slice input.(|l|) ((inputByteLen / r) * r) inputByteLen) (state_spec_v s).[l])
+
+(* absorb *)
+
+val absorb_lemma_l:
+  #a:keccak_alg
+  -> #m:m_spec{is_supported m}
+  -> s:state_spec m
+  -> r:size_nat{r > 0 /\ r <= 200}
+  -> inputByteLen:nat
+  -> input:multiseq (lanes m) inputByteLen
+  -> delimitedSuffix:byte_t
+  -> l:nat{l < lanes m} ->
+  Lemma
+   ((state_spec_v (absorb #a #m s r inputByteLen input delimitedSuffix)).[l] ==
+    Spec.absorb (state_spec_v s).[l] r inputByteLen input.(|l|) delimitedSuffix)
+
+(* squeeze_inner *)
+
+val squeeze_inner_lemma_l:
+  #a:keccak_alg
+  -> #m:m_spec{is_supported m}
+  -> r:size_nat{r > 0 /\ r <= 200}
+  -> outputByteLen:size_nat
+  -> i:size_nat{i < outputByteLen / r}
+  -> s:state_spec m
+  -> b:multiseq (lanes m) outputByteLen
+  -> s_pre:lseq uint8 (i * r)
+  -> l:nat{l < lanes m} ->
+  Lemma
+  (requires
+    s_pre == sub #uint8 #outputByteLen b.(|l|) 0 (i * r))
+  (ensures
+    (let s', b' = squeeze_inner #a #m r outputByteLen i (s, b) in
+    let s'_s, b'_s = Spec.squeeze_inner r outputByteLen i (state_spec_v s).[l] in
+    (state_spec_v s').[l] == s'_s /\ i * r + r <= outputByteLen /\
+    sub #uint8 #outputByteLen b'.(|l|) 0 (i * r + r) == Seq.append s_pre b'_s))
+
+(* squeeze_nblocks *)
+
+val lemma_generate_squeeze_inner_loop:
+    #a:keccak_alg
+  -> #m:m_spec{is_supported m}
+  -> r:size_nat{r > 0 /\ r <= 200}
+  -> outputByteLen:size_nat
+  -> n:nat{n <= outputByteLen}
+  -> s:state_spec m
+  -> b:multiseq (lanes m) outputByteLen
+  -> l:nat{l < lanes m} -> Lemma
+  (n / r <= outputByteLen / r /\
+   (let c (i:nat{i <= outputByteLen / r}) = Spec.state in
+   let (s1, out1) = generate_blocks r (outputByteLen / r) (n / r) c (Spec.squeeze_inner r outputByteLen) (state_spec_v s).[l] in
+   let (s2, out2) = repeat_gen (n / r) (squeeze_s m r outputByteLen) (squeeze_inner #a #m r outputByteLen) (s, b) in
+   (state_spec_v s2).[l] == (s1 <: Spec.state) /\ (n / r) * r <= outputByteLen /\
+   sub #uint8 #outputByteLen out2.(|l|) 0 ((n / r) * r) == out1))
+
+val squeeze_nblocks_lemma_l:
+    #a:keccak_alg
+  -> #m:m_spec{is_supported m}
+  -> r:size_nat{r > 0 /\ r <= 200}
+  -> outputByteLen:size_nat
+  -> s:state_spec m
+  -> b:multiseq (lanes m) outputByteLen
+  -> l:nat{l < lanes m} -> Lemma
+  (let c (i:nat{i <= outputByteLen / r}) = Spec.state in
+   let (s1, out1) = generate_blocks r (outputByteLen / r) (outputByteLen / r) c (Spec.squeeze_inner r outputByteLen) (state_spec_v s).[l] in
+   let (s2, out2) = repeat_gen (outputByteLen / r) (squeeze_s m r outputByteLen) (squeeze_inner #a #m r outputByteLen) (s, b) in
+   (state_spec_v s2).[l] == (s1 <: Spec.state) /\ (outputByteLen / r) * r <= outputByteLen /\
+   sub #uint8 #outputByteLen out2.(|l|) 0 ((outputByteLen / r) * r) == out1)
+
+(* squeeze_last *)
+
+val squeeze_last_lemma_l:
+  #a:keccak_alg
+  -> #m:m_spec{is_supported m}
+  -> r:size_nat{r > 0 /\ r <= 200}
+  -> outputByteLen:size_nat
+  -> s:state_spec m
+  -> b:multiseq (lanes m) outputByteLen
+  -> l:nat{l < lanes m} ->
+  Lemma
+   (let outRem = outputByteLen % r in
+    let b' = squeeze_last #a #m s r outputByteLen b in
+    let b'_s = Spec.storeState outRem (state_spec_v s).[l] in
+    outRem <= outputByteLen /\
+    sub #uint8 #outputByteLen b'.(|l|) (outputByteLen - outRem) outRem == b'_s /\
+    (forall i. (i < outputByteLen - outRem) ==>
+      Seq.index b'.(|l|) i == Seq.index b.(|l|) i))
+
+(* squeeze *)
+
+val squeeze_lemma_l:
+  #a:keccak_alg
+  -> #m:m_spec{is_supported m}
+  -> s:state_spec m
+  -> r:size_nat{r > 0 /\ r <= 200}
+  -> outputByteLen:size_nat
+  -> b:multiseq (lanes m) outputByteLen
+  -> l:nat{l < lanes m} ->
+  Lemma
+   ((squeeze #a #m s r outputByteLen b).(|l|) ==
+      Spec.squeeze (state_spec_v s).[l] r outputByteLen)
+
+(* keccak *)
+
+val keccak_lemma_l:
+  #a:keccak_alg
+  -> #m:m_spec{is_supported m}
+  -> rate:size_nat{rate % 8 == 0 /\ rate / 8 > 0 /\ rate <= 1600}
+  -> inputByteLen:nat
+  -> input:multiseq (lanes m) inputByteLen
+  -> delimitedSuffix:byte_t
+  -> outputByteLen:size_nat
+  -> b:multiseq (lanes m) outputByteLen
+  -> l:nat{l < lanes m} ->
+  Lemma
+   ((keccak #a #m rate inputByteLen input delimitedSuffix outputByteLen b).(|l|) ==
+      Spec.keccak rate (1600 - rate) inputByteLen input.(|l|) delimitedSuffix outputByteLen)
+
+(* shake128 *)
+
+val shake128_lemma_l:
+  m:m_spec{is_supported m}
+  -> inputByteLen:nat
+  -> input:multiseq (lanes m) inputByteLen
+  -> outputByteLen:size_nat
+  -> output:multiseq (lanes m) outputByteLen
+  -> l:nat{l < lanes m} ->
+  Lemma
+   ((shake128 m inputByteLen input outputByteLen output).(|l|) ==
+      Spec.shake128 inputByteLen input.(|l|) outputByteLen)
+
+(* shake256 *)
+
+val shake256_lemma_l:
+  m:m_spec{is_supported m}
+  -> inputByteLen:nat
+  -> input:multiseq (lanes m) inputByteLen
+  -> outputByteLen:size_nat
+  -> output:multiseq (lanes m) outputByteLen
+  -> l:nat{l < lanes m} ->
+  Lemma
+   ((shake256 m inputByteLen input outputByteLen output).(|l|) ==
+      Spec.shake256 inputByteLen input.(|l|) outputByteLen)
+
+(* sha3_224 *)
+
+val sha3_224_lemma_l:
+  m:m_spec{is_supported m}
+  -> inputByteLen:nat
+  -> input:multiseq (lanes m) inputByteLen
+  -> output:multiseq (lanes m) 28
+  -> l:nat{l < lanes m} ->
+  Lemma
+   ((sha3_224 m inputByteLen input output).(|l|) ==
+      Spec.sha3_224 inputByteLen input.(|l|))
+
+(* sha3_256 *)
+
+val sha3_256_lemma_l:
+  m:m_spec{is_supported m}
+  -> inputByteLen:nat
+  -> input:multiseq (lanes m) inputByteLen
+  -> output:multiseq (lanes m) 32
+  -> l:nat{l < lanes m} ->
+  Lemma
+   ((sha3_256 m inputByteLen input output).(|l|) ==
+      Spec.sha3_256 inputByteLen input.(|l|))
+
+(* sha3_384 *)
+
+val sha3_384_lemma_l:
+  m:m_spec{is_supported m}
+  -> inputByteLen:nat
+  -> input:multiseq (lanes m) inputByteLen
+  -> output:multiseq (lanes m) 48
+  -> l:nat{l < lanes m} ->
+  Lemma
+   ((sha3_384 m inputByteLen input output).(|l|) ==
+      Spec.sha3_384 inputByteLen input.(|l|))
+
+(* sha3_512 *)
+
+val sha3_512_lemma_l:
+  m:m_spec{is_supported m}
+  -> inputByteLen:nat
+  -> input:multiseq (lanes m) inputByteLen
+  -> output:multiseq (lanes m) 64
+  -> l:nat{l < lanes m} ->
+  Lemma
+   ((sha3_512 m inputByteLen input output).(|l|) ==
+      Spec.sha3_512 inputByteLen input.(|l|))
